src/basicmodal/language.lean
@@ -1,3 +1,7 @@
+/-
+Copyright (c) 2021 Paula Neeley. All rights reserved.
+Author: Paula Neeley
+-/
 
 inductive form : Type
   | bot  : form
