src/basicmodal/semantics/consistency.lean
@@ -1,5 +1,7 @@
--- Following the textbook "Dynamic Epistemic Logic" by 
--- Hans van Ditmarsch, Wiebe van der Hoek, and Barteld Kooi
+/-
+Copyright (c) 2021 Paula Neeley. All rights reserved.
+Author: Paula Neeley
+-/
 
 import basicmodal.language basicmodal.syntax.syntax 
 import basicmodal.semantics.semantics basicmodal.syntax.syntaxlemmas
@@ -10,8 +12,10 @@ open prfK
 
 ---------------------- Consistency ----------------------
 
+
 def sem_cons (AX : ctx) := ¬ global_sem_csq AX ⊥ 
 attribute [class] sem_cons
+
 
 lemma sem_consK : sem_cons ∅ :=
 begin
@@ -28,6 +32,7 @@ split, intros φ y h1,
 exact false.elim h1, use x, 
 rw forces, trivial 
 end
+
 
 lemma sem_consT : sem_cons T_axioms :=
 begin
@@ -46,6 +51,7 @@ exact rfl, use x,
 rw forces, trivial
 end
 
+
 lemma sem_consS4 : sem_cons S4_axioms :=
 begin
 rw sem_cons, rw global_sem_csq, push_neg,
@@ -57,7 +63,7 @@ use f, let v := λ n x, true,
 use v, let x := 42,
 split, 
 intros φ y h1,
-rw S4_axioms at h1, cases h1,
+cases h1,
 cases h1 with ψ h1, subst h1,
 intro h1, apply h1 y,
 exact rfl,
@@ -68,6 +74,7 @@ simp at *, exact h1,
 use x,
 rw forces, trivial
 end
+
 
 lemma sem_consS5 : sem_cons S5_axioms :=
 begin
@@ -80,7 +87,7 @@ use f, let v := λ n x, true,
 use v, let x := 42,
 split, 
 intros φ y h1,
-rw S5_axioms at h1, cases h1,
+cases h1,
 cases h1 with ψ h1, subst h1,
 intro h1, apply h1 y,
 exact rfl,
@@ -101,6 +108,7 @@ rw ←not_imp_not at h2, exact h2},
 apply h1, exact hax
 end
 
+
 lemma prnot_to_notpr (φ : form) (AX : ctx) (hax : sem_cons AX) : 
   prfK AX (¬φ) → ¬ prfK AX φ :=
 begin
@@ -110,6 +118,7 @@ have h4 : ¬ prfK AX ⊥, from nprfalse AX hax,
 exact absurd h3 h4
 end 
 
+
 lemma pr_to_notprnot (φ : form) (AX : ctx) (hax : sem_cons AX) : 
   prfK AX φ → ¬ prfK AX (¬φ) :=
 begin
@@ -117,22 +126,23 @@ have h1 : prfK AX (¬φ) → ¬ prfK AX φ, from prnot_to_notpr φ AX hax,
 rw ←not_imp_not at h1, intro h2, apply h1, rw not_not, exact h2,
 end 
 
--- finite conjunction of formulas
+
+-- Finite conjunction of formulas
 def fin_conj : list form → form
   | []  := ⊤
   | (φ::φs) := φ & (fin_conj φs)
 
--- a few helper lemmas about finite conjunctions
+
+-- A few helper lemmas about finite conjunctions
 lemma fin_conj_simp {Γ : ctx} : ∀ ψ : form, prfK Γ (¬fin_conj [ψ, ¬ψ]) :=
 begin
-intro ψ, simp, rw fin_conj, rw fin_conj, rw fin_conj, simp,
+intro ψ,
 have h2 : (prfK Γ (((¬ψ)&⊤) ↔ (¬ψ)) → 
   (prfK Γ (¬(ψ & ((¬ψ)&⊤))) ↔ prfK Γ (¬(ψ & (¬ψ))))), 
   from not_and_subst,
-simp at h2,
-specialize h2 phi_and_true, cases h2,
-exact h2_mpr not_contra
+exact (h2 phi_and_true).mpr not_contra
 end
+
 
 lemma imp_conj_imp_imp {Γ : ctx} {φ ψ χ : form} {L : list form} : 
   prfK Γ ((fin_conj (φ::L)) ⊃ ψ) ↔ prfK Γ (fin_conj L ⊃ (φ ⊃ ψ)) :=
@@ -142,11 +152,13 @@ intro h, dsimp [fin_conj] at h, rw and_right_imp at h, exact h,
 intro h, dsimp [fin_conj], rw and_right_imp, exact h
 end
 
+
 lemma fin_conj_cons_imp {Γ : ctx} {φ b : form} {L : list form} : 
  prfK Γ (fin_conj (φ::L) ⊃ (φ ⊃ b)) → prfK Γ (fin_conj L ⊃ (φ ⊃ b)) :=
 begin
 intro h, rw imp_conj_imp_imp at h, rw imp_imp_iff_imp at h, exact h, exact φ,
 end
+
 
 lemma fin_conj_append {Γ : ctx} {L L' : list form} :
   prfK Γ ((fin_conj L' & fin_conj L) ↔ (fin_conj (L' ++ L))) :=
@@ -158,59 +170,59 @@ exact mp (mp pl4 (cut (mp pl5 and_commute) (imp_and_imp (mp pl5 L'_ih))))
   (cut iden (cut (imp_and_imp (mp pl6 L'_ih)) (mp pl6 and_commute)))
 end 
 
+
 lemma fin_conj_empty {AX : ctx} {L : list form} (hax : sem_cons AX) :
   L = [] → ¬ prfK AX (fin_conj L ⊃ ⊥) :=
 begin
-intro h1, subst h1, rw fin_conj, simp at *,
+intro h1, subst h1,
 have h1 : prfK AX (¬⊥), from iden,
-simp at *, by_contradiction h2,
+by_contradiction h2,
 have h3 : prfK AX ⊥, from mp h2 h1,
 have h4 : ¬ prfK AX ⊥, from nprfalse AX hax,
 exact absurd h3 h4
 end 
+
 
 lemma fin_conj_repeat_helper {AX : ctx} {θ : form} {L : list form} (hax : sem_cons AX) :
   (∀ ψ ∈ L, ψ = θ) → prfK AX (θ ⊃ fin_conj L) :=
 begin
 intros h1, induction L,
 exact mp pl1 iden,
-rw fin_conj, simp at *,
+simp at *,
 cases h1 with h1 h2,
-specialize L_ih h2, subst h1,
-exact cut (mp double_imp pl4) (imp_and_and_imp (mp (mp pl4 iden) L_ih)),
+subst h1,
+exact cut (mp double_imp pl4) (imp_and_and_imp (mp (mp pl4 iden) (L_ih h2))),
 end
+
 
 lemma fin_conj_repeat {AX : ctx} {φ : form} {L : list form} (hax : sem_cons AX) :
   (∀ ψ ∈ L, ψ = ¬φ) → prfK AX (¬fin_conj L) → prfK AX φ :=
 begin
 intros h1 h2, induction L,
-rw fin_conj at h2,
 have h3 := mp dne h2,
 have h4 := nprfalse AX hax,
 exact absurd h3 h4,
-repeat {rw fin_conj at *}, simp at *,
+simp at *,
 cases h1 with h1 h3, 
-have h5 : prfK AX ((¬fin_conj L_tl) ⊃ ¬(¬φ)), from contrapos.mpr (fin_conj_repeat_helper hax h3),
+have h5 := contrapos.mpr (fin_conj_repeat_helper hax h3),
 subst h1,
 exact (mp (mp pl3 (contrapos.mpr (cut h5 dne))) 
   (contrapos.mpr (cut ((demorgans.mp) (mp (mp pl6 (iff_not and_switch)) h2)) dne)))
 end
+
 
 lemma fin_conj_box2 {AX : ctx} {φ ψ : form} : prfK AX ((□φ & □ψ) ⊃ □(φ & ψ)) :=
 begin
 exact (mp double_imp (cut2 pl6 (cut pl5 (cut (mp kdist (nec pl4)) kdist))))
 end
 
+
 lemma fin_conj_boxn {AX : ctx} {L : list form} : 
   prfK AX ((fin_conj (list.map □ L)) ⊃ (□(fin_conj L))) :=
 begin
 induction L,
-rw fin_conj, simp at *, rw fin_conj,
 exact (mp pl1 (nec prtrue)),
-rw list.map, repeat {rw fin_conj},
-have h1 := imp_and_imp,
-specialize h1 L_ih,
-exact (cut h1 fin_conj_box2)
+exact (cut (imp_and_imp L_ih) fin_conj_box2)
 end
 
 
@@ -219,21 +231,20 @@ lemma listempty {Γ : ctx} {L : list form} :
 begin
 intros h1 h2,
 by_contradiction h3,
-have h4 : L ≠ [] → 0 < L.length, from list.length_pos_of_ne_nil,
+have h4 := list.length_pos_of_ne_nil,
 specialize h4 h3,
-have h5 : 0 < L.length → ∃ a, a ∈ L, from list.exists_mem_of_length_pos,
+have h5 := list.exists_mem_of_length_pos,
 specialize h5 h4,
-cases h5 with φ h5, specialize h1 φ h5,
-have h6 : Γ = ∅ → ∀ φ, φ ∉ Γ, from set.eq_empty_iff_forall_not_mem.mp,
-specialize h6 h2, specialize h6 φ, exact absurd h1 h6
+cases h5 with φ h5,
+exact absurd (h1 φ h5) (set.eq_empty_iff_forall_not_mem.mp h2 φ)
 end
 
 
--- consistency for a finite set of formulas L
+-- Consistency for a finite set of formulas L
 def fin_ax_consist (AX : ctx) (L : list form) := ¬ prfK AX (fin_conj L ⊃ ⊥)
 
 
--- consistency for an arbitrary set of formulas Γ
+-- Consistency for an arbitrary set of formulas Γ
 def ax_consist (AX Γ : ctx) :=
   ∀ L : list form, (∀ ψ ∈ L, ψ ∈ Γ) → fin_ax_consist AX L
 
@@ -245,15 +256,11 @@ def max_ax_consist (AX Γ : ctx) :=
 
 lemma max_imp_ax {AX Γ : ctx} : max_ax_consist AX Γ → ax_consist AX Γ :=
 begin
-intro h1, rw max_ax_consist at h1, cases h1, exact h1_left
+intro h1, exact h1.left
 end
 
 
-/-Lemma: for every Gamma, phi, for every list L, for every formula b, 
-if everything in L is in Gamma or equal to phi, and you can prove conj L ⊃ b, 
-then there is a list L', such that everything in L' is in Gamma, and you can 
-prove conj L' ⊃ (phi ⊃ b)
--/
+-- Lemma 5 from class notes
 lemma five_helper (AX : ctx) : 
   ∀ Γ : ctx, ∀ φ : form, ∀ L : list form, ∀ b : form, 
   (∀ ψ ∈ L, ψ ∈ Γ ∨ ψ = φ) → prfK AX (fin_conj L ⊃ b) → ∃ L',
@@ -264,87 +271,73 @@ revert b,
 induction L,
 {intros b h2, existsi ([] : list form), split, 
 intros ψ h3, exfalso, apply list.not_mem_nil ψ h3, 
-dsimp [fin_conj] at *, exact imp_if_imp_imp h2},
+exact imp_if_imp_imp h2},
 {intros b h2,
 have h1a : ∀ (ψ : form), ψ ∈ L_tl → ψ ∈ Γ ∨ ψ = φ, 
-  {intros ψ h2, specialize h1 ψ, 
-  have h3 := list.subset_cons L_hd L_tl,
-  have h4 := list.mem_cons_of_mem L_hd h2, 
-  apply h1 h4},
-specialize L_ih h1a,
-have h1b: L_hd ∈ Γ ∨ L_hd = φ, 
-  {apply h1 L_hd, left, refl},
+{intros ψ h2, apply h1 ψ (list.mem_cons_of_mem L_hd h2)},
+have h1b : L_hd ∈ Γ ∨ L_hd = φ, 
+{apply h1 L_hd, left, refl},
 cases h1b, 
 have h3 : prfK AX (fin_conj L_tl ⊃ (L_hd ⊃ b)), 
   from and_right_imp.mp h2,
-specialize L_ih (L_hd ⊃ b) h3,
-cases L_ih with L' ih, existsi (L_hd::L' : list form),
+cases L_ih h1a (L_hd ⊃ b) h3 with L' ih, existsi (L_hd::L' : list form),
 cases ih, split, intros ψ h4, cases h4, 
 subst h4, exact h1b, 
 apply ih_left ψ h4, rw imp_shift at ih_right,
 rw ←imp_conj_imp_imp at ih_right, exact ih_right,
 have h3 : prfK AX (fin_conj (L_hd::L_tl) ⊃ b), 
 exact h2, exact b,
-specialize L_ih (φ ⊃ b),
-have h5 : prfK AX (fin_conj (L_hd :: L_tl) ⊃ b) → 
-  prfK AX (fin_conj L_tl ⊃ (L_hd ⊃ b)), 
-  from and_right_imp.mp,
-specialize h5 h2,
+have h5 := and_right_imp.mp,
 have h6 : prfK AX (fin_conj L_tl ⊃ (φ ⊃ b)), 
-  from eq.subst h1b h5,
-specialize L_ih h6, cases L_ih with L' ih, 
-cases ih, existsi (L' : list form), split, 
-exact ih_left, exact imp_imp_iff_imp.mp ih_right}
+  from eq.subst h1b (h5 h2),
+cases L_ih h1a (φ ⊃ b) h6 with L' ih, 
+existsi (L' : list form), split, 
+exact ih.left, exact imp_imp_iff_imp.mp ih.right}
 end
 
--- Lemma 5 from class notes
+
 lemma five (AX : ctx) : 
   ∀ Γ : ctx, ∀ φ : form, ¬ ax_consist AX (Γ un φ) → ∃ L',
   (∀ ψ ∈ L', ψ ∈ Γ) ∧ prfK AX (fin_conj L' ⊃ ¬φ) :=
 begin
-intro Γ, intro φ, intro h1, simp at *, rw ax_consist at h1, 
+intro Γ, intro φ, intro h1, rw ax_consist at h1, 
 push_neg at h1,
 cases h1 with L h1,
 have h2 : (∀ ψ ∈ L, ψ ∈ Γ ∨ ψ = φ) → prfK AX (fin_conj L ⊃ ⊥) → ∃ L',
   (∀ ψ ∈ L', ψ ∈ Γ) ∧ prfK AX (fin_conj L' ⊃ (φ ⊃ ⊥)), from five_helper AX Γ φ L ⊥,
 cases h1,
 have h3 : (∀ (ψ : form), ψ ∈ L → ψ ∈ Γ ∨ ψ = φ), 
-{intros ψ this, specialize h1_left ψ this, exact or.swap h1_left},
-specialize h2 h3, apply h2, rw fin_ax_consist at h1_right, rw not_not at h1_right,
+{intros ψ this, exact or.swap (h1_left ψ this)},
+apply h2 h3, rw fin_ax_consist at h1_right, rw not_not at h1_right,
 exact h1_right,
 end
 
 
+-- Lemma 6 from class notes
 lemma six_helper (AX Γ : ctx) (h : ax_consist AX Γ) :
 max_ax_consist AX Γ → ∀ φ : form, φ ∈ Γ ∨ (¬φ) ∈ Γ :=
 begin
-intros h1 φ, simp, rw or_iff_not_and_not, by_contradiction h2,
-cases h2 with h2l h2r, rw max_ax_consist at h1,
-cases h1 with h1l h1r, clear h, 
+intros h1 φ, rw or_iff_not_and_not, by_contradiction h2,
+cases h2 with h2l h2r,
+cases h1 with h1l h1r,
 have h2 := h1r (Γ un φ), have h3 := h1r (Γ un ¬φ),
-simp at h3, have h4 : ¬ax_consist AX (Γ un ¬φ), 
+have h4 : ¬ax_consist AX (Γ un ¬φ), 
 {apply h3, from set.ssubset_insert h2r},
 have h5 : ¬ax_consist AX (Γ un φ), 
-{simp at *, apply h2, from set.ssubset_insert h2l}, 
-clear h2 h3, simp at *, have h6 := five AX Γ φ _, have h7 := five AX Γ (¬φ) _, 
-cases h6 with L' h6, cases h7 with L h7, dsimp at *, cases h6 with h6l h6r,
+{apply h2, from set.ssubset_insert h2l}, 
+clear h2 h3, have h6 := five AX Γ φ _, have h7 := five AX Γ (¬φ) _, 
+cases h6 with L' h6, cases h7 with L h7, cases h6 with h6l h6r,
 cases h7 with h7l h7r,
-have h8 : prfK AX ((fin_conj L' & fin_conj L) ⊃ ((¬φ) & ¬¬φ)), 
-from imp_and_and_imp (mp (mp pl4 h6r) h7r),
-simp at h8,
-rw ax_consist at h1l,
-have h12: prfK AX ((fin_conj (L' ++ L)) ⊃ ⊥), 
-from cut (mp pl6 fin_conj_append) (cut h8 (mp pl5 contra_equiv_false)),
-specialize h1l (L' ++ L), rw fin_ax_consist at h1l,
-have h13: (∀ (ψ : form), ψ ∈ L' ++ L → ψ ∈ Γ), 
-intro ψ, specialize h6l ψ, specialize h7l ψ, intro h13,
-rw list.mem_append at h13, cases h13, exact h6l h13, exact h7l h13,
-specialize h1l h13, exact absurd h12 h1l,
-exact h4,
-exact h5,
+have h8 := imp_and_and_imp (mp (mp pl4 h6r) h7r),
+have h12 := cut (mp pl6 fin_conj_append) (cut h8 (mp pl5 contra_equiv_false)),
+have h13 : (∀ (ψ : form), ψ ∈ L' ++ L → ψ ∈ Γ), 
+{intros ψ h13, rw list.mem_append at h13, 
+cases h13, exact (h6l ψ) h13, exact (h7l ψ) h13},
+exact absurd h12 ((h1l (L' ++ L)) h13),
+exact h4, exact h5
 end
 
--- lemma 6 from class notes
+
 lemma six (AX Γ : ctx) (h : ax_consist AX Γ) :
 max_ax_consist AX Γ ↔ ∀ φ, (φ ∈ Γ ∨ (¬φ) ∈ Γ) ∧ ¬(φ ∈ Γ ∧ (¬φ) ∈ Γ) :=
 begin 
@@ -353,14 +346,13 @@ intro h1, intro φ,
 split, exact six_helper AX Γ h h1 φ,
 {rw ←not_and, by_contradiction h2,
 cases h2 with h2 h3,
-rw ax_consist at h,
 specialize h ([φ, ¬φ]), simp at *,
 have h4 : (∀ (ψ : form), ψ = φ ∨ ψ = ¬φ → ψ ∈ Γ), 
 {intros ψ h4, simp at *, cases h4, subst h4, exact h2, subst h4, exact h3},
 specialize h h4, rw fin_ax_consist at h, 
 have h5 : prfK AX (¬fin_conj [φ, ¬φ]), from fin_conj_simp φ, 
 exact absurd h5 h},
-intro h1, rw max_ax_consist, split, exact h,
+intro h1, split, exact h,
 intros Γ' h2,
 have h3 : Γ ⊆ Γ' ∧ ¬ Γ' ⊆ Γ, from h2,
 cases h3,
@@ -378,6 +370,8 @@ subst h7, exact h6, rw fin_ax_consist, rw not_not,
 exact fin_conj_simp ψ
 end
 
+
+-- Exercise 1 from class notes
 lemma ex1help {AX Γ : ctx} {φ : form} {L L' : list form} :
   (∀ ψ ∈ L, ψ ∈ Γ) → prfK AX (fin_conj L ⊃ φ) → (∀ ψ ∈ L', ψ ∈ (insert φ Γ)) 
   → ∃ L'' : list form, (∀ ψ ∈ L'', ψ ∈ Γ) ∧ prfK AX (fin_conj L'' ⊃ fin_conj L') :=
@@ -388,8 +382,7 @@ split,
 intros ψ h4, exact false.elim h4,
 exact iden,
 simp at *, cases h3 with h3 h4,
-specialize L'_ih h4,
-cases L'_ih with L'' L'_ih,
+cases L'_ih h4 with L'' L'_ih,
 cases L'_ih with ih1 ih2,
 cases h3, 
 existsi (L''++L : list form),
@@ -405,12 +398,12 @@ split, simp at *, split, exact h3, exact ih1,
 exact imp_and_imp ih2
 end
 
+
 lemma exercise1 {AX Γ : ctx} {φ : form} {L : list form} :
   max_ax_consist AX Γ → (∀ ψ ∈ L, ψ ∈ Γ) → prfK AX (fin_conj L ⊃ φ) → φ ∈ Γ :=
 begin
 intros h1 h2 h3, 
 by_contradiction h4, 
-rw max_ax_consist at h1,
 cases h1 with h1 h5, 
 specialize h5 (Γ ∪ {φ}), 
 simp at h5,
@@ -421,13 +414,13 @@ cases h5 with L' h5,
 cases h5 with h5 h6,
 rw fin_ax_consist at h6, 
 rw not_not at h6,
-rw ax_consist at h1, 
 have h7 := ex1help h2 h3 h5,
 cases h7 with L'' h7,
 cases h7 with h7 h8,
-specialize h1 L'' h7, apply h1,
+apply h1 L'' h7,
 exact cut h8 h6
 end
+
 
 lemma max_dn (AX Γ : ctx) (h : max_ax_consist AX Γ) (φ : form) :
   φ ∈ Γ ↔ (¬¬φ) ∈ Γ :=
@@ -435,14 +428,13 @@ begin
 split, intro h1, 
 have h2 : (∀ ψ ∈ [φ], ψ ∈ Γ) → prfK AX (fin_conj [φ] ⊃ (¬¬φ)) → (¬¬φ) ∈ Γ, from exercise1 h,
 simp at *, apply h2, exact h1,
-repeat {rw fin_conj},
 exact (cut (mp pl5 phi_and_true) dni), 
 intro h1,
 have h2 : (∀ ψ ∈ [¬¬φ], ψ ∈ Γ) → prfK AX (fin_conj [¬¬φ] ⊃ φ) → φ ∈ Γ, from exercise1 h,
 simp at *, apply h2, exact h1,
-repeat {rw fin_conj},
 exact (cut (mp pl5 phi_and_true) dne), 
 end
+
 
 lemma max_boxdn (AX Γ : ctx) (h : max_ax_consist AX Γ) (φ : form) :
   (¬□φ) ∈ Γ → (¬□(¬¬φ)) ∈ Γ :=
@@ -451,26 +443,26 @@ intro h1,
 have h2 : (∀ ψ ∈ [(¬□φ)], ψ ∈ Γ) → prfK AX (fin_conj [(¬□φ)] ⊃ (¬□(¬¬φ))) → (¬□(¬¬φ)) ∈ Γ, 
   from exercise1 h,
 simp at *, apply h2, exact h1, clear h2,
-repeat {rw fin_conj at *},
 exact (cut (mp pl5 phi_and_true) (mp pl5 box_dn)), 
 end
+
 
 lemma max_notiff (AX Γ : ctx) (h : max_ax_consist AX Γ) (φ : form) :
   φ ∉ Γ ↔ (¬φ) ∈ Γ :=
 begin
 split, intro h1,
-have h2 : ax_consist AX Γ, from max_imp_ax h, 
-have h3 : ∀ φ : form, φ ∈ Γ ∨ (¬φ) ∈ Γ, from six_helper AX Γ h2 h,
+have h2 := max_imp_ax h, 
+have h3 := six_helper AX Γ h2 h,
 specialize h3 φ, cases h3, exact absurd h3 h1, exact h3,
 intro h1,
-have h2 : ax_consist AX Γ, from max_imp_ax h, 
-have h3 : max_ax_consist AX Γ ↔ ∀ φ, (φ ∈ Γ ∨ (¬φ) ∈ Γ) ∧ ¬(φ ∈ Γ ∧ (¬φ) ∈ Γ), 
-  from six AX Γ h2,
+have h2 := max_imp_ax h, 
+have h3 := six AX Γ h2,
 cases h3, specialize h3_mp h (¬φ), simp at *,
-cases h3_mp with mp1 mp2, specialize mp2 h1,
-have h4 : φ ∈ Γ ↔ (¬¬φ) ∈ Γ, from max_dn AX Γ h φ,
-rw ←not_iff_not at h4, cases h4, apply h4_mpr, exact mp2
+cases h3_mp with mp1 mp2,
+have h4 := max_dn AX Γ h φ,
+rw ←not_iff_not at h4, apply h4.mpr, exact mp2 h1
 end
+
 
 lemma max_imp_1 {AX Γ : ctx} {φ ψ : form} : 
   max_ax_consist AX Γ → (φ ∈ Γ → ψ ∈ Γ) → (φ ⊃ ψ) ∈ Γ :=
@@ -480,15 +472,12 @@ cases h2,
 have h3 : (∀ χ ∈ [¬φ], χ ∈ Γ) → prfK AX (fin_conj [¬φ] ⊃ (φ ⊃ ψ)) → (φ ⊃ ψ) ∈ Γ, from exercise1 h1,
 simp at *, apply h3, 
 exact (max_notiff AX Γ h1 φ).mp h2,
-repeat {rw fin_conj at *},
-simp at *,
-have h4 : prfK AX ((¬φ) ⊃ (φ ⊃ ψ)), from and_right_imp.mp exfalso,
-simp at *,
-exact cut (mp pl5 phi_and_true) h4,
+exact cut (mp pl5 phi_and_true) (and_right_imp.mp exfalso),
 have h3 : (∀ χ ∈ [ψ], χ ∈ Γ) → prfK AX (fin_conj [ψ] ⊃ (φ ⊃ ψ)) → (φ ⊃ ψ) ∈ Γ, from exercise1 h1,
 simp at *, 
 apply h3, exact h2, exact (cut (mp pl5 phi_and_true) pl1),
 end
+
 
 lemma max_imp_2 {AX Γ : ctx} {φ ψ : form} : 
   max_ax_consist AX Γ → (φ ⊃ ψ) ∈ Γ → φ ∈ Γ → ψ ∈ Γ :=
@@ -496,24 +485,21 @@ begin
 intros h1 h2 h3,
 have h4 : (∀ χ ∈ [φ, (φ ⊃ ψ)], χ ∈ Γ) → prfK AX (fin_conj [φ, (φ ⊃ ψ)] ⊃ ψ) → ψ ∈ Γ, from exercise1 h1,
 simp at *, apply h4, intros χ h5, cases h5, subst h5, exact h3, subst h5, exact h2,
-repeat {rw fin_conj}, simp at *,
 exact and_right_imp.mpr (mp pl5 phi_and_true)
 end
+
 
 lemma max_conj_1 {AX Γ : ctx} {φ ψ : form} : 
   max_ax_consist AX Γ → (φ ∈ Γ ∧ ψ ∈ Γ) → (φ & ψ) ∈ Γ :=
 begin
-intros h1 h2, cases h2,
+intros h1 h2,
 have h3 : (∀ χ ∈ [φ], χ ∈ Γ) → prfK AX (fin_conj [φ] ⊃ (ψ ⊃ (φ & ψ))) → (ψ ⊃ (φ & ψ)) ∈ Γ, 
   from exercise1 h1,
-simp at *, specialize h3 h2_left,
-repeat {rw fin_conj at *},
-have h5 : prfK AX ((φ&¬⊥)⊃(ψ⊃φ&ψ)),
-exact (cut (mp pl5 phi_and_true) pl4), 
-specialize h3 h5,
-have h6 : (ψ ⊃ (φ & ψ)) ∈ Γ → ψ ∈ Γ → (φ & ψ) ∈ Γ, from max_imp_2 h1,
-apply h6, exact h3, exact h2_right
+simp at *,
+apply max_imp_2 h1, 
+exact h3 h2.left (cut (mp pl5 phi_and_true) pl4), exact h2.right
 end
+
 
 lemma max_conj_2 {AX Γ : ctx} {φ ψ : form} : 
   max_ax_consist AX Γ → (φ & ψ) ∈ Γ → φ ∈ Γ :=
@@ -521,9 +507,10 @@ begin
 intros h1 h2,
 have h3 : (∀ χ ∈ [(φ & ψ)], χ ∈ Γ) → prfK AX (fin_conj [(φ & ψ)] ⊃ φ) → φ ∈ Γ, 
   from exercise1 h1,
-simp at *, apply h3, exact h2, repeat {rw fin_conj},
+simp at *, apply h3, exact h2,
 exact (cut (mp pl5 phi_and_true) pl5)
 end
+
 
 lemma max_conj_3 {AX Γ : ctx} {φ ψ : form} : 
   max_ax_consist AX Γ → (φ & ψ) ∈ Γ → ψ ∈ Γ :=
@@ -531,27 +518,23 @@ begin
 intros h1 h2,
 have h3 : (∀ χ ∈ [(φ & ψ)], χ ∈ Γ) → prfK AX (fin_conj [(φ & ψ)] ⊃ ψ) → ψ ∈ Γ, 
   from exercise1 h1,
-simp at *, apply h3, exact h2, repeat {rw fin_conj},
+simp at *, apply h3, exact h2,
 exact (cut (mp pl5 phi_and_true) pl6)
 end
 
--- Γ is maximally AX-consistent iff it is AX-consistent and for 
--- every AX-consistent set Γ', if Γ ⊆ Γ', then Γ = Γ'
 lemma max_equiv (AX Γ : ctx) : max_ax_consist AX Γ ↔ ax_consist AX Γ ∧ 
   ∀ Γ', ax_consist AX Γ' → Γ ⊆ Γ' → Γ = Γ' :=
 begin
 split, 
-{intro h1, split, rw max_ax_consist at h1, exact h1.left, 
+{intro h1, split, exact h1.left, 
 intros Γ' h2 h3, rw set.subset.antisymm_iff, split, exact h3,
-by_contradiction h4, rw max_ax_consist at h1, cases h1, 
-have h5 := and.intro h3 h4, 
-have h6 : Γ ⊂ Γ', from h5,
-specialize h1_right Γ' h6, exact h1_right h2}, 
-intro h1, cases h1, rw max_ax_consist, split, exact h1_left,
-intros Γ' h2, by_contradiction h3, specialize h1_right Γ' h3,
-rw set.ssubset_def at h2, cases h2, apply h2_right, rw h1_right h2_left
+by_contradiction h4,
+exact h1.right Γ' (and.intro h3 h4) h2}, 
+intro h1, split, exact h1.left,
+intros Γ' h2, by_contradiction h3,
+rw set.ssubset_def at h2, apply h2.right, 
+rw h1.right Γ' h3 h2.left,
 end
-
 
 
 open zorn
@@ -563,11 +546,10 @@ lemma lindenhelper (c : set ctx) (h : c.nonempty) (h1 : chain (⊆) c) (L : list
 begin
 intro h2,
 induction L, simp,
-rw ←set.nonempty_def, exact h,
+exact h,
 have h2b : ∀ φ, φ ∈ L_tl → φ ∈ ⋃₀(c), 
 {intros φ h3, apply h2, exact set.mem_union_right (eq φ) h3},
-specialize L_ih h2b,
-cases L_ih with m ih,
+cases L_ih h2b with m ih,
 cases ih with h3 ih,
 specialize h2 L_hd, 
 simp at h2,
@@ -577,41 +559,32 @@ existsi (m' ∪ m : ctx),
 have h5 : m' ∪ m ∈ c, 
 {have h6 := chain.total_of_refl h1 h3 h2,
 cases h6,
-have h7 := set.union_eq_self_of_subset_right h6,
-exact (eq.substr h7 h2), 
-have h7 := set.union_eq_self_of_subset_left h6,
-exact (eq.substr h7 h3)},
+exact (eq.substr (set.union_eq_self_of_subset_right h6) h2), 
+exact (eq.substr (set.union_eq_self_of_subset_left h6) h3)},
 existsi (h5 : m' ∪ m ∈ c),
 intros ψ h6, cases h6,
 subst h6, exact set.mem_union_left m h4,
-specialize ih ψ h6, exact set.mem_union_right m' ih
+exact set.mem_union_right m' (ih ψ h6)
 end
 
 
 lemma lindenbaum (AX Γ : ctx) (hax : ax_consist AX Γ) : 
   ∃ Γ', max_ax_consist AX Γ' ∧ Γ ⊆ Γ' :=
 begin
-let P := { Γ'' | Γ'' ⊇ Γ ∧ ax_consist AX Γ''},
+let P := { Γ'' | Γ'' ⊇ Γ ∧ ax_consist Γ''},
 have h : ∀ c ⊆ P, chain (⊆) c → c.nonempty → ∃ub ∈ P, ∀ s ∈ c, s ⊆ ub, 
 {intros c h2 h3 h4, use ⋃₀(c), 
 have h5 := lindenhelper c h4 h3,
-split, 
-split,
-rw superset,
-rw set.nonempty_def at h4,
+repeat {split}, 
 cases h4 with Γ'' h4,
 have h6 := set.mem_of_mem_of_subset h4 h2,
 cases h6 with h6 h7,
-rw superset at h6,
 apply set.subset_sUnion_of_subset c Γ'' h6 h4,
-rw ax_consist,
 intros L h6,
-specialize h5 L h6,
-cases h5 with m h5,
+cases h5 L h6 with m h5,
 cases h5 with h7 h5,
-have h8 := set.mem_of_mem_of_subset h7 h2,
-cases h8 with h8 h9,
-rw ax_consist at h9, apply h9, exact h5,
+cases (set.mem_of_mem_of_subset h7 h2) with h8 h9,
+apply h9, exact h5,
 intros s h7, exact set.subset_sUnion_of_mem h7},
 have h1 : Γ ∈ P,
 split,
@@ -621,18 +594,20 @@ cases zorn_subset₀ P h Γ h1 with Γ' h2,
 cases h2 with h2 h3,
 cases h3 with h3 h4,
 use Γ', split, rw max_equiv, split, apply h2.2, 
-intros m h5 h6, symmetry, apply h4 m, split, apply set.subset.trans h2.1 h6,
+intros m h5 h6, symmetry, apply h4 m, split, 
+apply set.subset.trans h2.1 h6,
 exact h5, exact h6, apply h2.1
 end
 
--- Corollary 8
+
+-- Corollary 8 from class notes
 lemma max_ax_exists (AX : ctx) (hax : sem_cons AX) : ∃ Γ : ctx, max_ax_consist AX Γ :=
 begin
 have h1 : ax_consist AX ∅,
-{rw ax_consist, intro L, intro h2, rw fin_ax_consist, 
+{intro L, intro h2, rw fin_ax_consist, 
 have h3 := listempty h2, have this : ∅ = ∅, refl, 
 specialize h3 this, subst h3, by_contradiction h4, 
-have h5 := mp dne, apply nprfalse AX hax, exact h5 h4},
-have h2 : ∃ Γ, max_ax_consist AX Γ ∧ ∅ ⊆ Γ, from lindenbaum AX ∅ h1, 
+apply nprfalse AX hax, exact mp dne h4},
+have h2 := lindenbaum AX ∅ h1, 
 cases h2 with Γ h2, cases h2 with h2 h3, existsi (Γ : ctx), apply h2
 end
