src/basicmodal/semantics/definability.lean
@@ -1,12 +1,14 @@
--- Following the textbook "Dynamic Epistemic Logic" by 
--- Hans van Ditmarsch, Wiebe van der Hoek, and Barteld Kooi
+/-
+Copyright (c) 2021 Paula Neeley. All rights reserved.
+Author: Paula Neeley
+-/
 
 import basicmodal.language basicmodal.syntax.syntax 
 import basicmodal.semantics.semantics basicmodal.paths
 import data.set.basic
+local attribute [instance] classical.prop_decidable
 
 open form
-local attribute [instance] classical.prop_decidable
 
 
 ---------------------- Frame Definability ----------------------
@@ -19,37 +21,29 @@ def defines (φ : form) (F : set (frame)) :=
 
 ---------------------- Definability Proofs ----------------------
 
-section
-open classical
-open set
-
 variable f : frame
 variables {α : Type} (r : α → α → Prop)
 
-def euclidean := ∀ ⦃x y z⦄, r x y → r x z → r y z 
-
-def ref_class : set (frame) := { f : frame | reflexive (f.rel) }
-def symm_class : set (frame) := { f : frame | symmetric (f.rel) }
-def trans_class : set (frame) := { f : frame | transitive (f.rel) }
-def euclid_class : set (frame) := { f : frame | euclidean (f.rel) }
-def equiv_class : set (frame) := { f : frame | equivalence (f.rel) }
+def euclidean       := ∀ ⦃x y z⦄, r x y → r x z → r y z 
+def ref_class       : set (frame) := { f : frame | reflexive (f.rel)   }
+def symm_class      : set (frame) := { f : frame | symmetric (f.rel)   }
+def trans_class     : set (frame) := { f : frame | transitive (f.rel)  }
+def euclid_class    : set (frame) := { f : frame | euclidean (f.rel)   }
+def equiv_class     : set (frame) := { f : frame | equivalence (f.rel) }
 def ref_trans_class : set (frame) := ref_class ∩ trans_class
+
 
 lemma equiv_ref_euclid (f : frame) : f ∈ equiv_class ↔ f ∈ (ref_class ∩ euclid_class) :=
 begin
-rw equiv_class, rw ref_class, rw euclid_class,
-rw set.mem_set_of_eq, simp, rw equivalence, split,
+split,
 intro h1, cases h1 with h1 h2, cases h2 with h2 h3,
-split, exact h1, rw euclidean, intros x y z h4 h5,
-rw symmetric at h2, specialize h2 h4, rw transitive at h3,
-exact h3 h2 h5,
+split, exact h1, 
+intros x y z h4 h5, exact h3 (h2 h4) h5,
 intro h1, split, cases h1, exact h1_left,
-split, cases h1 with h1 h2, rw symmetric,
-intros x y h3, rw euclidean at h2, rw reflexive at h1,
-specialize h1 x, exact h2 h3 h1,
-rw transitive, intros x y z h2 h3, cases h1 with h1 h4,
-rw euclidean at h4, rw reflexive at h1,
-specialize h1 x, have h5 := h4 h2 h1, exact h4 h5 h3
+split, cases h1 with h1 h2,
+intros x y h3, exact h2 h3 (h1 x),
+intros x y z h2 h3, cases h1 with h1 h4,
+exact h4 (h4 h2 (h1 x)) h3
 end
 
 
@@ -75,14 +69,13 @@ lemma symm_helper : ∀ φ f, f ∈ symm_class → f_valid (φ ⊃ (□ (◇φ))
 begin
 dsimp, intros φ f h v x h1 y h2 h3,
 by_contradiction h4,
-specialize h3 x, have h4 := h h2, 
-have h5 := h3 h4, exact h5 h1
+exact ((h3 x) (h h2)) h1
 end
 
 
 theorem symm_def : defines ((p 0) ⊃ (□ (◇ (p 0)))) (symm_class) :=
 begin
-simp, rw defines, intro f, split,
+intro f, split,
 {exact symm_helper (p 0) f},
 {intro h1, by_contradiction h2, rw symm_class at h2,
 rw set.nmem_set_of_eq at h2, rw symmetric at h2,
@@ -92,8 +85,7 @@ cases h2 with y h2,
 let v := λ n x, n = 0 ∧ ¬ f.rel y x,
 specialize h1 v x,
 simp [forces, v] at h1,
-specialize h1 h2.right y h2.left, 
-apply h1,
+apply h1 h2.right y h2.left,
 intros y1 h3 h4, exact absurd h3 h4}
 end
 
@@ -101,21 +93,16 @@ end
 lemma trans_helper : ∀ φ f, f ∈ trans_class → f_valid (□ φ ⊃ □ (□ φ)) f :=
 begin
 intros φ f h v x h1 y h3 z h4, 
-have h5 := h h3, have h6 := h5 h4,
-specialize h1 z, apply h1 h6
+exact (h1 z) ((h h3) h4)
 end
 
 
 lemma euclid_helper : ∀ φ f, f ∈ euclid_class → f_valid (◇ φ ⊃ □ (◇ φ)) f :=
 begin
-dsimp, intros φ f h v x h1 y h2 h3,
+intros φ f h v x h1 y h2 h3,
 apply h1, intros z h4,
-have h6 := h h2, specialize h6 h4,
-clear h, specialize h3 z h6, exact h3
+exact h3 z ((h h2) h4)
 end
 
-
-
-end
 
 
