src/basicmodal/semantics/semantics.lean
@@ -1,19 +1,26 @@
+/-
+Copyright (c) 2021 Paula Neeley. All rights reserved.
+Author: Paula Neeley
+-/
+
 import basicmodal.language basicmodal.syntax.syntax
 import logic.basic data.set.basic
 local attribute [instance] classical.prop_decidable
 
-
 open form
+
 
 ---------------------- Semantics ----------------------
 
--- definition of relational frame
+
+-- Definition of relational frame
 structure frame :=
 (states : Type)
 (h : inhabited states)
 (rel : states → states → Prop)
 
--- definition of forces
+
+-- Definition of forces
 def forces (f : frame) (v : nat → f.states → Prop) : f.states → form → Prop
   | x (bot)    := false
   | x (var n)  := v n x
@@ -21,60 +28,62 @@ def forces (f : frame) (v : nat → f.states → Prop) : f.states → form → P
   | x (impl φ ψ) := (forces x φ) → (forces x ψ)
   | x (box φ)  := ∀ y, f.rel x y → forces y φ
 
+
 -- φ is valid in a model M = (f,v)
 def m_valid (φ : form) (f : frame) 
   (v : nat → f.states → Prop) := 
   ∀ x, forces f v x φ
 
+
 -- φ is valid in a frame f
 def f_valid (φ : form) (f : frame) := 
   ∀ v x, forces f v x φ
+
 
 -- φ is valid in a class of frames F
 def F_valid (φ : form) (F : set (frame)) := 
   ∀ f ∈ F, ∀ v x, forces f v x φ
 
+
 -- φ is universally valid (valid in all frames)
 def u_valid (φ : form) := 
   ∀ f v x, forces f v x φ
+
 
 -- A context is true at a world in a model if each 
 -- formula of the context is true at that world in that model
 def forces_ctx (f : frame) (v : nat → f.states → Prop) 
   (Γ : ctx) := ∀ φ, ∀ x, φ ∈ Γ → forces f v x φ
 
+
 -- Global semantic consequence
 def global_sem_csq (Γ : ctx) (φ : form) :=
   ∀ f v, forces_ctx f v Γ → ∀ x, forces f v x φ
+
 
 lemma not_forces_imp :  ∀ f v x φ, 
   (¬(forces f v x φ)) ↔ (forces f v x (¬φ)) :=
 begin
 intros f v x φ, split, 
-{intros h1 h2, exact h1 h2},
-{intros h1 h2, specialize h1 h2, exact h1}
+repeat {intros h1 h2, exact h1 h2},
 end
+
 
 lemma forces_exists {f : frame} {v : nat → f.states → Prop} {x : f.states} {φ : form} :
   forces f v x (◇φ) ↔ ∃ y : f.states, (f.rel x y ∧ forces f v y φ) :=
 begin
-simp at *,
-split,
-intro h1,
-rw forces at h1, rw forces at h1,
+split, intro h1,
+repeat {rw forces at h1},
 have h2 := not_or_of_imp h1,
-clear h1, cases h2, push_neg at h2,
+cases h2, push_neg at h2,
 cases h2 with y h2, cases h2 with h2 h3,
 existsi (y : f.states), split, exact h2,
 have h4 := (not_forces_imp f v y (¬φ)).mp h3,
 repeat {rw forces at h4}, repeat {rw imp_false at h4},
 rw not_not at h4, exact h4,
-rw forces at h2, exact false.elim h2,
+exact false.elim h2,
 intro h1, cases h1 with y h1,
 cases h1 with h1 h2,
-rw forces,
 intro h3,
-rw forces at h3, specialize h3 y h1,
-rw ←not_forces_imp at h3, 
-exact absurd h2 h3
+exact absurd h2 (h3 y h1)
 end
