src/basicmodal/semantics/undefinability.lean
@@ -1,13 +1,14 @@
--- Following the textbook "Dynamic Epistemic Logic" by 
--- Hans van Ditmarsch, Wiebe van der Hoek, and Barteld Kooi
+/-
+Copyright (c) 2021 Paula Neeley. All rights reserved.
+Author: Paula Neeley
+-/
 
 import basicmodal.language basicmodal.syntax.syntax 
 import basicmodal.semantics.semantics data.set.basic basicmodal.paths 
 import basicmodal.semantics.definability
-
-open form
 local attribute [instance] classical.prop_decidable
 
+open form
 
 
 ---------------------- Frame Undefinability ----------------------
@@ -31,10 +32,12 @@ def frame.rel.dunion (r1 : α → α → Prop) (r2 : β → β → Prop) :
   | (sum.inr b1) (sum.inr b2) := r2 b1 b2
   | _ _                       := false
 
+
 def val_dunion {f1 f2 : frame} (v1 : nat → f1.states → Prop) 
   (v2 : nat → f2.states → Prop) : nat → (sum f1.states f2.states) → Prop
   | n (sum.inl x1) := v1 n x1
   | n (sum.inr x2) := v2 n x2
+
 
 def frame.dunion (f1 f2 : frame) : frame :=
 {
@@ -43,30 +46,26 @@ def frame.dunion (f1 f2 : frame) : frame :=
   rel := frame.rel.dunion (f1.rel) (f2.rel)
 }
 
+
 theorem invariance_dunion (f1 f2 : frame) (v1 : nat → f1.states → Prop) 
   (v2 : nat → f2.states → Prop) (x1 : f1.states) : 
   theory_at f1 v1 x1 = theory_at (f1.dunion f2) (val_dunion v1 v2) (sum.inl x1) :=
 begin
 ext φ, revert x1, induction φ,
-{intro x1, split, repeat {intro h, rw theory_at at *, exact h}},
-{intro x1, split, repeat {intro h, rw theory_at at *, exact h}},
-{rename φ_φ φ, rename φ_ψ ψ, rename φ_ih_φ ih_φ, rename φ_ih_ψ ih_ψ, 
-intro x1, split, intro h, split, specialize ih_φ x1, 
-cases ih_φ, cases h, exact ih_φ_mp h_left,
-specialize ih_ψ x1, cases ih_ψ, cases h, exact ih_ψ_mp h_right,
-intro h, split, specialize ih_φ x1, cases ih_φ, cases h, exact ih_φ_mpr h_left,
-specialize ih_ψ x1, cases ih_ψ, cases h, exact ih_ψ_mpr h_right},
-{rename φ_φ φ, rename φ_ψ ψ, rename φ_ih_φ ih_φ, rename φ_ih_ψ ih_ψ,
-intro x1, split, intro h, specialize ih_φ x1, cases ih_φ, specialize ih_ψ x1,
-cases ih_ψ, intro h1, have h2 := ih_φ_mpr h1, have h3 := h h2, exact ih_ψ_mp h3, 
-intro h, specialize ih_φ x1, specialize ih_ψ x1, cases ih_φ, cases ih_ψ, 
-intro h1, have h2 := ih_φ_mp h1, have h3 := h h2, exact ih_ψ_mpr h3},
-{rename φ_φ φ, intro x1, split, intros h s h1, cases s, specialize φ_ih s, 
-cases φ_ih, specialize h s, have h2 := h h1, exact φ_ih_mp h2,
-apply false.elim h1, intros h s h1, specialize φ_ih s, cases φ_ih,
-specialize h (sum.inl s), have h2 := h h1, exact φ_ih_mpr h2}
+repeat {rename φ_ih_φ ih_φ},
+repeat {rename φ_ih_ψ ih_ψ},
+repeat {rename φ_φ φ},
+repeat {rename φ_ψ ψ},
+repeat {intro x1},
+repeat {split},
+repeat {intro h, exact h},
+{intro h, split, exact (ih_φ x1).mp h.left, exact (ih_ψ x1).mp h.right},
+{intro h, split, exact (ih_φ x1).mpr h.left, exact (ih_ψ x1).mpr h.right},
+{intros h h1, exact (ih_ψ x1).mp (h ((ih_φ x1).mpr h1))}, 
+{intros h h1, exact (ih_ψ x1).mpr (h ((ih_φ x1).mp h1))},
+{intros h s h1, cases s, exact (φ_ih s).mp ((h s) h1), exact false.elim h1},
+{intros h s h1, exact (φ_ih s).mpr ((h (sum.inl s)) h1)}
 end
-
 
 
 -- Invariance under generated submodels
@@ -77,36 +76,33 @@ def frame.gen_subframe (f : frame) (x : f.states) : frame :=
   rel := λ x1 x2, (f.rel) x1.val x2.val
 }
 
+
 def val_gen_subframe (f : frame) (x : f.states)
   (v : nat → f.states → Prop) : nat → (frame.gen_subframe f x).states → Prop :=
   λ n, λ y, v n y.val
+
 
 theorem invariance_gen_submodel (f : frame) (v : ℕ → f.states → Prop) 
   (x : f.states) (y : (frame.gen_subframe f x).states) :
   theory_at f v y.val = theory_at (f.gen_subframe x) (val_gen_subframe f x v) y :=
 begin
 ext φ, revert y, induction φ,
-{intro y, split, repeat {intro h1, exact h1}}, 
-{intro y, split, repeat {intro h1, exact h1}},
-{rename φ_ih_φ ih_φ, rename φ_ih_ψ ih_ψ, rename φ_φ φ, 
-rename φ_ψ ψ, intro y, specialize ih_φ y, specialize ih_ψ y, 
-cases ih_φ, cases ih_ψ, split, intro h1, cases h1, split, 
-exact ih_φ_mp h1_left, exact ih_ψ_mp h1_right, intro h1, 
-cases h1, split, exact ih_φ_mpr h1_left, exact ih_ψ_mpr h1_right}, 
-{rename φ_φ φ, rename φ_ψ ψ, rename φ_ih_φ ih_φ, 
-rename φ_ih_ψ ih_ψ, intro y, specialize ih_φ y, specialize ih_ψ y, 
-cases ih_φ, cases ih_ψ, split, intros h1 h2, have h3 := ih_φ_mpr h2, 
-have h4 := h1 h3, exact ih_ψ_mp h4, intros h1 h2, 
-have h3 := ih_φ_mp h2, have h4 := h1 h3, exact ih_ψ_mpr h4},
-{rename φ_φ φ, intro y, split, {intros h1 z h2, specialize φ_ih z,
-cases φ_ih, specialize h1 z.val, have h3 := h1 h2, exact φ_ih_mp h3}, 
-{intro h1, intros z h2, 
-have h3 := reach_right x y.val z f.rel (and.intro y.property h2),
-specialize φ_ih ⟨z, h3⟩, cases φ_ih, specialize h1 ⟨z, h3⟩, 
-have h4 := h1 h2, exact φ_ih_mpr h4}}
+repeat {rename φ_ih_φ ih_φ},
+repeat {rename φ_ih_ψ ih_ψ},
+repeat {rename φ_φ φ},
+repeat {rename φ_ψ ψ},
+repeat {intro y},
+repeat {split},
+repeat {intro h1, exact h1}, 
+{intro h1, split, exact (ih_φ y).mp h1.left, exact (ih_ψ y).mp h1.right}, 
+{intro h1, split, exact (ih_φ y).mpr h1.left, exact (ih_ψ y).mpr h1.right}, 
+{intros h1 h2, exact (ih_ψ y).mp (h1 ((ih_φ y).mpr h2))}, 
+{intros h1 h2, exact (ih_ψ y).mpr (h1 ((ih_φ y).mp h2))},
+{intros h1 z h2, exact (φ_ih z).mp ((h1 z.val) h2)}, 
+{intros h1 z h2, 
+have h3 := reach_right x y.1 z f.rel (and.intro y.2 h2),
+exact (φ_ih ⟨z, h3⟩).mpr ((h1 ⟨z, h3⟩) h2)}
 end
-
-
 
 
 -- Invariance under bisimulation
@@ -114,18 +110,22 @@ def base {f1 f2 : frame} (v1 : nat → f1.states → Prop)
   (v2 : nat → f2.states → Prop) (x1 : f1.states) (x2 : f2.states) := 
   ∀ n, v1 n x1 ↔ v2 n x2
 
+
 def forth {f1 f2 : frame} (bisim : f1.states → f2.states → Prop) 
   (x1 : f1.states) (x2 : f2.states) := 
   ∀ y1, f1.rel x1 y1 → (∃ y2 : f2.states, f2.rel x2 y2 ∧ bisim y1 y2)
+
 
 def back {f1 f2 : frame} (bisim : f1.states → f2.states → Prop) 
   (x1 : f1.states) (x2 : f2.states) := 
   ∀ y2, f2.rel x2 y2 → (∃ y1 : f1.states, f1.rel x1 y1 ∧ bisim y1 y2)
 
+
 -- Bisimulation between M1 = (f1,v1) and M2 = (f2,v2)
 def is_bisimulation {f1 f2 : frame} (v1 : nat → f1.states → Prop) 
   (v2 : nat → f2.states → Prop) (bisim : f1.states → f2.states → Prop) := ∀ x1 x2,
   bisim x1 x2 → (base v1 v2 x1 x2 ∧ forth bisim x1 x2 ∧ back bisim x1 x2)
+
 
 theorem invariance_bisim {f1 f2 : frame} (v1 : nat → f1.states → Prop) 
   (v2 : nat → f2.states → Prop) (bisim : f1.states → f2.states → Prop) 
@@ -133,35 +133,37 @@ theorem invariance_bisim {f1 f2 : frame} (v1 : nat → f1.states → Prop)
   bisim x1 x2 → theory_at f1 v1 x1 = theory_at f2 v2 x2 :=
 begin
 intro h1, ext φ, revert x1 x2, induction φ,
-{intros x1 x2 h1, split, intro h2, exact h2, intro h2, exact h2}, 
-{intros x1 x2 h1, specialize h x1 x2 h1, cases h, 
-specialize h_left φ, cases h_left, split, intro h2, 
-exact h_left_mp h2, intro h2, exact h_left_mpr h2}, 
-{intros x1 x2 h1, specialize φ_ih_φ x1 x2 h1, specialize φ_ih_ψ x1 x2 h1, 
-cases φ_ih_φ, cases φ_ih_ψ, split, intro h2, cases h2, split, 
-exact φ_ih_φ_mp h2_left, exact φ_ih_ψ_mp h2_right, intro h2, 
-cases h2, split, exact φ_ih_φ_mpr h2_left, exact φ_ih_ψ_mpr h2_right}, 
-{intros x1 x2 h1, specialize φ_ih_φ x1 x2 h1, specialize φ_ih_ψ x1 x2 h1,
-cases φ_ih_φ, cases φ_ih_ψ, split, intros h2 h3, have h4 := φ_ih_φ_mpr h3,
-have h5 := h2 h4, exact φ_ih_ψ_mp h5, intros h2 h3, have h4 := φ_ih_φ_mp h3,
-have h5 := h2 h4, exact φ_ih_ψ_mpr h5},
-{rename φ_φ φ, intros x1 x2 h1, specialize h x1 x2 h1, cases h with h4 h5,
+repeat {rename φ_ih_φ ih_φ},
+repeat {rename φ_ih_ψ ih_ψ},
+repeat {rename φ_φ φ},
+repeat {rename φ_ψ ψ},
+repeat {intros x1 x2 h1},
+{split, repeat {intro h2, exact h2}}, 
+{split, 
+intro h2, exact ((h x1 x2 h1).left φ).mp h2, 
+intro h2, exact ((h x1 x2 h1).left φ).mpr h2}, 
+{split, 
+intro h2, split, exact (ih_φ x1 x2 h1).mp h2.left, exact (ih_ψ x1 x2 h1).mp h2.right, 
+intro h2, split, exact (ih_φ x1 x2 h1).mpr h2.left, exact (ih_ψ x1 x2 h1).mpr h2.right}, 
+{split, 
+intros h2 h3, exact (ih_ψ x1 x2 h1).mp (h2 ((ih_φ x1 x2 h1).mpr h3)), 
+intros h2 h3, exact (ih_ψ x1 x2 h1).mpr (h2 ((ih_φ x1 x2 h1).mp h3))},
+{cases h x1 x2 h1 with h4 h5,
 cases h5 with h5 h6, split,
-{intros h2 y2 h3, specialize h6 y2 h3, cases h6 with y1 h6, 
-cases h6 with h6 h7, specialize h2 y1 h6, specialize φ_ih y1 y2 h7, 
-cases φ_ih, exact φ_ih_mp h2},
-{intros h2 y1 h3, specialize h5 y1 h3, cases h5 with y2 h5, 
-cases h5 with h5 h7, specialize h2 y2 h5, specialize φ_ih y1 y2 h7, 
-cases φ_ih, exact φ_ih_mpr h2}}
+{intros h2 y2 h3, cases h6 y2 h3 with y1 h6, 
+cases h6 with h6 h7, exact (φ_ih y1 y2 h7).mp (h2 y1 h6)},
+{intros h2 y1 h3, cases h5 y1 h3 with y2 h5, 
+cases h5 with h5 h7, exact (φ_ih y1 y2 h7).mpr (h2 y2 h5)}}
 end
-
 
 
 -- Invariance using surjective bounded morphisms
 open function
 
+
 def is_bddmorphism {f1 f2 : frame} (g : f1.states → f2.states) := 
   ∀ x1 : f1.states, forth (λ x1 x2, (g x1) = x2) x1 (g x1) ∧ back (λ x1 x2, (g x1) = x2) x1 (g x1)
+
 
 def is_surjbddmorphism {f1 f2 : frame} (g : f1.states → f2.states) 
   := surjective g ∧ is_bddmorphism g
@@ -175,21 +177,22 @@ push_neg at h1, push_neg,
 cases h1 with v2 h1,
 cases h1 with y h1,
 let v1 := (λ n x, v2 n (g x)), use v1,
-cases h with hl hr, specialize hl y, cases hl with x hl, 
+cases h with hl hr, cases hl y with x hl, 
 existsi (x : f1.states), have h3 := invariance_bisim v1 v2 (λ x y, g x = y),
 have h4 : is_bisimulation v1 v2 (λ (x : f1.states) (y : f2.states), g x = y), 
 {intros x1 x2 h2, split,
 {intro n, split, intro h, subst h2, apply h, intro h, subst h2, apply h},
-specialize hr x1, cases hr, split,
+split,
 have h5 : forth (λ (x1 : f1.states) (x2 : f2.states), g x1 = x2) x1 x2, 
-from eq.subst h2 hr_left, exact h5, 
+from eq.subst h2 (hr x1).left, exact h5, 
 have h5 : back (λ (x1 : f1.states) (x2 : f2.states), g x1 = x2) x1 x2,
-from eq.subst h2 hr_right, exact h5},
+from eq.subst h2 (hr x1).right, exact h5},
 specialize h3 h4 x y hl, intro h2, apply h1,
 rw set.subset.antisymm_iff at h3, cases h3, 
 rw set.subset_def at h3_left,
-specialize h3_left φ h2, exact h3_left,
+exact h3_left φ h2
 end
+
 
 lemma invariance_pull_back (F : set (frame)) {f1 f2 : frame} 
   (h1 : f1 ∈ F) (h2 : f2 ∉ F) : 
@@ -198,9 +201,6 @@ begin
 intro h, cases h with g h,
 intro φ, by_contradiction h3, 
 have h4 := h3 f1, specialize h3 f2, 
-rw ←not_iff_not at h3, cases h3,
-have h5 := h3_mp h2, 
-cases h4, have h7 := h4_mp h1, 
-have h8 := pull_back g h φ h5, 
-exact h8 h7
+rw ←not_iff_not at h3,
+exact (pull_back g h φ (h3.mp h2)) (h4.mp h1)
 end
