src/basicmodal/syntax/soundness.lean
@@ -1,11 +1,11 @@
--- Following the textbook "Dynamic Epistemic Logic" by 
--- Hans van Ditmarsch, Wiebe van der Hoek, and Barteld Kooi
+/-
+Copyright (c) 2021 Paula Neeley. All rights reserved.
+Author: Paula Neeley
+-/
 
 import basicmodal.language data.set.basic basicmodal.semantics.semantics 
 import basicmodal.semantics.definability basicmodal.syntax.syntaxlemmas
 local attribute [instance] classical.prop_decidable
-
-
 
 ---------------------- Soundness ----------------------
 
@@ -13,35 +13,29 @@ theorem soundness (AX : ctx) (φ : form) : prfK AX φ → global_sem_csq AX φ :
 begin
 intro h,
 induction h,
-{intros f v h x, rw forces_ctx at h,
-specialize h h_φ x, have h1 := h h_h, 
-exact h1},
+{intros f v h x,
+exact (h h_φ x) h_h},
 {intros f v x h2 h3 h4, exact h3}, 
 {intros f v x h2 h3 h4 h5, apply h3, 
 exact h5, apply h4, exact h5}, 
 {intros f x v h1 h2 h3,
 by_contradiction h4,
-specialize h2 h4, specialize h3 h4, 
-rw ← not_forces_imp at h2, exact h2 h3},
-{intros f v x h1 h2 h3, simp [forces] at *, 
+exact (h2 h4) (h3 h4)},
+{intros f v x h1 h2 h3,
 exact and.intro h2 h3},
 {intros f v x h1 h2, exact h2.left},
 {intros f v x h1 h2, exact h2.right},
-{intros f v x h1 h2 h3, rw forces at h2,
-rw forces at h2, rw forces at h2, rw forces at h2,
-rw imp_false at h2, rw imp_false at h2, rw not_imp_not at h2,
+{intros f v x h1 h2 h3, 
+repeat {rw forces at h2},
+repeat {rw imp_false at h2}, 
+rw not_imp_not at h2,
 exact h2 h3}, 
-{intros f v x h1 h2 h3, simp [forces] at *, 
-intros x' h4, specialize h3 x' h4,
-specialize h2 x' h4 h3, exact h2}, 
+{intros f v x h1 h2 h3 x' h4,
+exact h2 x' h4 (h3 x' h4)}, 
 {intros f v x h, 
-specialize h_ih_hpq f v x h,
-specialize h_ih_hp f v x h,
-exact h_ih_hpq h_ih_hp}, 
+exact (h_ih_hpq f v x h) (h_ih_hp f v x h)}, 
 {intros f v h1 x y h2,
-rw global_sem_csq at h_ih,
-specialize h_ih f v h1 y, 
-exact h_ih},
+exact h_ih f v h1 y},
 end
 
 
@@ -49,21 +43,20 @@ lemma soundnesshelper {Γ : ctx} {φ : form} {C : set (frame)} :
   prfK Γ φ → (∀ ψ ∈ Γ, F_valid ψ C) → F_valid φ C :=
 begin
 intros h1 h2 f h3 v, induction h1,
-{intro x, specialize h2 h1_φ h1_h, rw F_valid at h2, specialize h2 f h3 v x, exact h2},
+{intro x, exact h2 h1_φ h1_h f h3 v x},
 {intros x h4 h5, exact h4},
-{intros x h4 h5 h6, have h7 := h4 h6, have h8 := h5 h6, exact h7 h8},
-{intros x h3 h4, by_contradiction h5, specialize h3 h5, specialize h4 h5, 
-rw ← not_forces_imp at h3, exact h3 h4},
+{intros x h4 h5 h6, exact (h4 h6) (h5 h6)},
+{intros x h3 h4, by_contradiction h5, specialize h3 h5, 
+rw ←not_forces_imp at h3, exact h3 (h4 h5)},
 {intros x h4 h5, exact and.intro h4 h5}, 
 {intros x h4, exact h4.left}, 
 {intros x h4, exact h4.right}, 
-{intros x h4 h5, rw forces at h4, rw forces at h4,
-rw forces at h4, rw forces at h4, rw imp_false at h4,
-rw imp_false at h4, rw not_imp_not at h4, exact h4 h5},
-{intros x h3 h4, simp [forces] at *, intros x' h5, specialize h3 x' h5,
-specialize h4 x' h5, exact h3 h4},
-{intro x, specialize h1_ih_hp h2 x, specialize h1_ih_hpq h2 x h1_ih_hp, 
-exact h1_ih_hpq},
+{intros x h4 h5, repeat {rw forces at h4}, 
+repeat {rw imp_false at h4},
+rw not_imp_not at h4, exact h4 h5},
+{intros x h3 h4, intros x' h5,
+exact (h3 x' h5) (h4 x' h5)},
+{intro x, exact h1_ih_hpq h2 x (h1_ih_hp h2 x)},
 {intros x y h3, apply h1_ih, exact h2}
 end
 
@@ -71,12 +64,11 @@ end
 lemma inclusion_valid {C C' : set (frame)} : ∀ ψ, C ⊆ C' → F_valid ψ C' → F_valid ψ C :=
 begin
 intros φ h1 h2 f h3 v x, 
-have h4 := set.mem_of_subset_of_mem h1 h3,
-specialize h2 f h4 v x, exact h2
+exact h2 f (set.mem_of_subset_of_mem h1 h3) v x
 end
 
 
-def T_axioms : ctx := {φ : form | ∃ ψ, φ = (□ ψ ⊃ ψ)}
+def T_axioms  : ctx := {φ : form | ∃ ψ, φ = (□ ψ ⊃ ψ)}
 def S4_axioms : ctx := T_axioms ∪ {φ : form | ∃ ψ, φ = (□ ψ ⊃ □ (□ ψ))}
 def S5_axioms : ctx := T_axioms ∪ {φ : form | ∃ ψ, φ = (◇ ψ ⊃ □ (◇ ψ))}
 
@@ -88,10 +80,12 @@ cases h1 with ψ h1, subst h1,
 apply ref_helper, exact h2
 end
 
+
 theorem T_soundness (φ : form) : prfK T_axioms φ → F_valid φ ref_class :=
 begin
 intro h, apply soundnesshelper, apply h, apply T_helper 
 end
+
 
 lemma S4_helper : ∀ φ ∈ S4_axioms, F_valid φ ref_trans_class :=
 begin
@@ -103,10 +97,12 @@ cases h1 with h1 h3,
 apply trans_helper, exact h2r}
 end
 
+
 theorem S4_soundness (φ : form) : prfK S4_axioms φ → F_valid φ ref_trans_class :=
 begin
 intro h, apply soundnesshelper, apply h, apply S4_helper
 end
+
 
 lemma S5_helper : ∀ φ ∈ S5_axioms, F_valid φ equiv_class :=
 begin
@@ -117,12 +113,11 @@ cases h1 with h1 h3,
 {apply T_helper, exact h1, 
 exact h2l},
 {cases h3 with ψ h3, dsimp at h3,
-subst h3, apply euclid_helper, rw euclid_class,
-rw set.mem_set_of_eq, rw euclidean,
+subst h3, apply euclid_helper,
 intros x y z h1 h2,
-rw symmetric at h2r,
-specialize h2r h1, exact h2rr h2r h2}
+exact h2rr (h2r h1) h2}
 end
+
 
 theorem S5_soundness (φ : form) : prfK S5_axioms φ → F_valid φ equiv_class :=
 begin
