src/del/announcements.lean
@@ -1,23 +1,29 @@
--- Following the textbook "Dynamic Epistemic Logic" by 
--- Hans van Ditmarsch, Wiebe van der Hoek, and Barteld Kooi
+/-
+Copyright (c) 2021 Paula Neeley. All rights reserved.
+Author: Paula Neeley
+Following the textbook "Dynamic Epistemic Logic" by 
+Hans van Ditmarsch, Wiebe van der Hoek, and Barteld Kooi
+-/
 
 import del.languageDEL del.semantics.semanticsDEL 
 import data.set.basic data.equiv.basic
-variable {agents : Type}
 local attribute [instance] classical.prop_decidable
+
+variable {agents : Type}
 
 
 ---------------------- Facts about Announcements ----------------------
+
 
 -- Proposition 4.10, pg. 77
 lemma functional_announce (φ ψ : formPA agents) : 
   F_validPA ((¬(U φ (¬ψ))) ⊃ (U φ ψ)) equiv_class :=
 begin
-rw F_validPA, intros f h v x,
-rw forcesPA, intro h1,
+intros f h v x h1,
 rw forces_update_dual at h1,
 cases h1 with Ph1 h1, intro h, exact h1
 end
+
 
 -- Proposition 4.11, pg. 77
 lemma partial_announce (φ ψ : formPA agents) : 
@@ -43,13 +49,15 @@ split, intro h, intro h1, exact h1,
 rw forcesPA, trivial
 end
 
---prop 4.22
+
+--Proposition 4.22
 lemma public_annouce_var (φ : formPA agents) (f : frame agents) 
   (v : nat → f.states → Prop) (x : f.states) (n : ℕ) :
   forcesPA f v x (U φ p n) ↔ forcesPA f v x (φ ⊃ (p n)) :=
 begin
 split, repeat {intros h1 h2, exact h1 h2},
 end
+
 
 lemma public_annouce_conj (φ ψ χ : formPA agents) (f : frame agents) 
   (v : nat → f.states → Prop) (x : f.states) :
@@ -58,15 +66,16 @@ begin
 split,
 intro h1,
 split,
-intro h2, specialize h1 h2,
-exact h1.left,
-intro h2, specialize h1 h2,
-exact h1.right, 
+intro h2,
+exact (h1 h2).left,
+intro h2,
+exact (h1 h2).right, 
 intros h1 h2,
 split,
 exact h1.left h2,
 exact h1.right h2,
 end
+
 
 -- Proposition 4.12, pg. 77
 lemma public_announce_neg (φ ψ : formPA agents) (f : frame agents) 
@@ -83,6 +92,7 @@ intro h2, exact absurd h2 h1,
 intros h h2, apply h1, intro h3, exact h2
 end
 
+
 -- Proposition 4.18, pg. 79
 lemma public_announce_know (φ ψ : formPA agents) (f : frame agents) 
   (v : nat → f.states → Prop) (s : f.states) (a : agents) :
@@ -90,19 +100,11 @@ lemma public_announce_know (φ ψ : formPA agents) (f : frame agents)
 begin
 split,
 intros h1 h2 t hrel h3,
-rw forcesPA at h1,
-specialize h1 h2,
-rw forcesPA at h1,
-specialize h1 ⟨t, h3⟩,
-specialize h1 hrel,
-exact h1,
-intro h1,
-intro h2,
-rw forcesPA,
-rintro ⟨t, h3⟩,
-intro hrel,
+exact h1 h2 ⟨t, h3⟩ hrel,
+rintros h1 h2 ⟨t, h3⟩ hrel,
 exact h1 h2 t hrel h3,
 end
+
 
 namespace compositionPA
 
@@ -110,6 +112,7 @@ variables A A'     : Prop
 variable  B        : A → Prop
 variable  A''      : A' → Prop
 variable  B'       : ∀ h : A', A'' h → Prop
+
 
 lemma comp_helper1 (h : A ↔ ∃ h : A', A'' h) 
   (h' : ∀ (h1 : A) (h2 : A') (h3 : A'' h2), B h1 ↔ B' h2 h3) : 
@@ -123,6 +126,7 @@ begin
   cases h.mp h1 with h2 h3,
   exact (h' h1 h2 h3).mpr (hh h2 h3)
 end
+
 
 lemma comp_helper2 (φ ψ : formPA agents) (f : frame agents) 
   (v : nat → f.states → Prop) (s : f.states) :
@@ -143,24 +147,23 @@ intro h3,
 exact h2,
 end
 
--- lemmas from 12/02/2020 meeting start here --
 
 def is_frame_iso (f1 f2 : frame agents) (F : f1.states ≃ f2.states) := 
   ∀ x x' : f1.states, ∀ a : agents, (f1.rel a x x' ↔ f2.rel a (F x) (F x'))
 
+
 def is_model_iso (f1 f2 : frame agents) (v1 : nat → f1.states → Prop)
   (v2 : nat → f2.states → Prop) (F : f1.states ≃ f2.states) := 
   is_frame_iso f1 f2 F ∧ ∀ n, ∀ x : f1.states, v1 n x = v2 n (F x)
+
 
 lemma model_iso_symm {f1 f2 : frame agents} {v1 : nat → f1.states → Prop}
   {v2 : nat → f2.states → Prop} {F : f1.states ≃ f2.states} :
   is_model_iso f1 f2 v1 v2 F → is_model_iso f2 f1 v2 v1 (F.symm) :=
 begin
 intro h1,
-rw is_model_iso at *,
 cases h1 with h1 h2,
 split,
-rw is_frame_iso at *,
 intros x x' a,
 specialize h1 (F.inv_fun x) (F.inv_fun x') a, 
 simp at h1,
@@ -169,6 +172,7 @@ intros n x,
 specialize h2 n (F.inv_fun x), simp at *,
 exact h2.symm
 end
+
 
 def restrict_F {f1 f2 : frame agents} {v1 : nat → f1.states → Prop}
   {v2 : nat → f2.states → Prop} (F : f1.states ≃ f2.states) 
@@ -212,18 +216,12 @@ begin
 intros h1 φ h2 x h3 h4,
 cases h1 with h1 h6,
 split,
-intros x1 y1 a,
-cases x1 with x1 hx1,
-cases y1 with y1 hy1,
-rw is_frame_iso at h1,
-specialize h1 x1 y1 a,
-apply h1,
-intros n x1,
-dsimp,
-cases x1 with x1 hx1,
-specialize h6 n x1,
-apply h6,
+rintros ⟨x1, hx1⟩ ⟨y1, hy1⟩ a,
+apply h1 x1 y1 a,
+rintros n ⟨x1, hx1⟩,
+apply h6 n x1,
 end
+
 
 lemma comp_helper3 (f1 f2 : frame agents) (v1 : nat → f1.states → Prop)
   (v2 : nat → f2.states → Prop) (F : f1.states ≃ f2.states) :
@@ -233,8 +231,7 @@ begin
 intro h1,
 intros x1 φ, induction φ generalizing f1 v1 f2 v2 F h1 x1,
 split,
-repeat {intro h3,
-exact h3},
+repeat {intro h3, exact h3},
 split,
 repeat {intro h3,
 rename φ n,
@@ -250,7 +247,6 @@ repeat {rename φ_ih_ψ ψ_ih},
 repeat {rename φ_a a},
 split,
 repeat {intro h3,
-rw forcesPA at *,
 cases h3 with h3 h4,
 split},
 exact (φ_ih f1 v1 f2 v2 F h1 x1).mp h3,
@@ -265,54 +261,44 @@ split,
 intros h3 y1 h4,
 specialize φ_ih f1 v1 f2 v2 F h1 (F.inv_fun y1),
 cases h1 with h1 h5,
-rw is_frame_iso at h1,
-specialize h3 (F.inv_fun y1),
 specialize h1 x1 (F.inv_fun y1) a,
 simp at *,
-exact φ_ih.mp (h3 (h1.mpr h4)),
+exact φ_ih.mp (h3 (F.inv_fun y1) (h1.mpr h4)),
 intros h3 x2 h4,
 specialize φ_ih f1 v1 f2 v2 F h1 x2,
 cases h1 with h1 h5,
-rw is_frame_iso at h1,
-specialize h1 x1 x2 a,
-rw forcesPA at h3,
-specialize h3 (F.to_fun x2),
-simp at *,
-exact φ_ih.mpr (h3 (h1.mp h4)),
+exact φ_ih.mpr (h3 (F.to_fun x2) ((h1 x1 x2 a).mp h4)),
 split,
 intro h2,
 specialize φ_ih f1 v1 f2 v2 F h1,
 intro h3,
 have h4 := ((φ_ih x1).mpr h3),
 have h5 := update_iso F h1 φ φ_ih x1 h4 h3,
-rw forcesPA at h2,
-specialize h2 h4,
 specialize ψ_ih (f1.restrict (λ (y : f1.states), forcesPA f1 v1 y φ) x1 h4)
   (λ (n : ℕ) (u : (f1.restrict (λ (y : f1.states), forcesPA f1 v1 y φ) x1 h4).states), v1 n u.val)
   (f2.restrict (λ (y : f2.states), forcesPA f2 v2 y φ) (F x1) h3)
   (λ (n : ℕ) (u : (f2.restrict (λ (y : f2.states), forcesPA f2 v2 y φ) (F x1) h3).states), 
   v2 n u.val) (restrict_F F φ x1 φ_ih h4 h3) h5 ⟨x1, h4⟩,
-have h6 := ψ_ih.mp h2,
+have h6 := ψ_ih.mp (h2 h4),
 convert h6,
 intro h2,
 specialize φ_ih f1 v1 f2 v2 F h1,
 intro h3,
 have h4 := (φ_ih x1).mp h3,
-rw forcesPA at h2,
-specialize h2 h4,
 have h5 := update_iso F h1 φ φ_ih x1 h3 h4,
 specialize ψ_ih (f2.restrict (λ (y : f2.states), forcesPA f2 v2 y φ) (F x1) h4)
   (λ (n : ℕ) (u : (f2.restrict (λ (y : f2.states), forcesPA f2 v2 y φ) (F x1) h4).states), v2 n u.val)
   (f1.restrict (λ (y : f1.states), forcesPA f1 v1 y φ) x1 h3)
   (λ (n : ℕ) (u : (f1.restrict (λ (y : f1.states), forcesPA f1 v1 y φ) x1 h3).states), v1 n u.val) 
   (_) (model_iso_symm h5) ⟨F x1, h4⟩,
-have h6 := ψ_ih.mp h2,
+have h6 := ψ_ih.mp (h2 h4),
 convert h6,
 {exact (equiv.eq_symm_apply F).mpr rfl},
 end
 
+
 -- Proposition 4.17, pg. 78
-lemma public_announce_comp1 (φ ψ χ : formPA agents) (f : frame agents) 
+lemma public_announce_comp (φ ψ χ : formPA agents) (f : frame agents) 
   (v : nat → f.states → Prop) (s : f.states) :
   forcesPA f v s (U (φ & U φ ψ) χ) ↔ forcesPA f v s (U φ (U ψ χ)) :=
 begin
@@ -345,7 +331,6 @@ let F : (f.restrict (λ (y : f.states), forcesPA f v y (φ&φ.update ψ)) s h1).
   right_inv :=
   begin
     rintro ⟨⟨x, h4⟩, h5⟩,
-    dsimp,
     refl,
   end},
 have h4 := comp_helper3 (f.restrict (λ (y : f.states), forcesPA f v y (φ&φ.update ψ)) s h1)
@@ -370,20 +355,15 @@ have h5 : is_model_iso (f.restrict (λ (y : f.states), forcesPA f v y (φ&φ.upd
   forcesPA f v y φ) s h2).states), v n u.val) y ψ) ⟨s, h2⟩ h3).states), (λ (n : ℕ) (u : 
   (f.restrict (λ (y : f.states), forcesPA f v y φ) s h2).states), v n u.val) n u.val) F,
 {
-  clear h4,
   split,
-  intros x1 y1 a,
-  cases x1 with x1 hx1,
-  cases y1 with y1 hy1,
+  rintros ⟨x1, hx1⟩ ⟨y1, hy1⟩ a,
   refl,
-  intros n x,
-  cases x with x hx,
+  rintros n ⟨x, hx⟩,
   refl
 },
-specialize h4 h5,
-specialize h4 ⟨s, h1⟩ χ,
-convert h4
+convert h4 h5 ⟨s, h1⟩ χ
 end
+
 
 end compositionPA
 
