src/del/semantics/completenessDEL.lean
@@ -1,12 +1,23 @@
+/-
+Copyright (c) 2021 Paula Neeley. All rights reserved.
+Author: Paula Neeley
+Following the textbook "Dynamic Epistemic Logic" by 
+Hans van Ditmarsch, Wiebe van der Hoek, and Barteld Kooi
+-/
+
 import del.semantics.consistencyDEL del.syntax.soundnessDEL
 import data.list.basic
 local attribute [instance] classical.prop_decidable
 
+variables {agents : Type}
 open prfS5
 open S5lemma
-variables {agents : Type}
-namespace canonical
 
+
+---------------------- Canonical Model Construction ----------------------
+
+
+namespace canonical
 
 def canonical [hax : sem_cons (∅ : ctx agents) equiv_class] : frame agents := 
 { 
@@ -15,8 +26,10 @@ def canonical [hax : sem_cons (∅ : ctx agents) equiv_class] : frame agents :=
   rel := λ a, λ xΓ yΔ, ∀ φ : form agents, K a φ ∈ xΓ.val → φ ∈ yΔ.val
 }
 
+
 def val_canonical [hax : sem_cons (∅ : ctx agents) equiv_class] : 
   nat → canonical.states → Prop := λ n, λ xΓ : canonical.states, (form.var n) ∈ (xΓ.val : ctx agents)
+
 
 lemma existence (hax : sem_cons (∅ : ctx agents) equiv_class) (xΓ : canonical.states) :
   ∀ a, ∀ φ : form agents, (¬ K a (¬φ)) ∈ xΓ.val ↔ ∃ yΔ : canonical.states, φ ∈ yΔ.val ∧ canonical.rel a xΓ yΔ :=
@@ -30,15 +43,14 @@ have h3 := five Γbox φ h2,
 cases h3 with L h3, cases h3 with h3 h4,
 have h5 := cut fin_conj_boxn (mp kdist (nec h4)),
 have h6 := exercise1,
-specialize h6 xΓ.2,
 have h7 : ∀ ψ ∈ (list.map (form.box a) L), ψ ∈ xΓ.1, 
 intros ψ h8, simp at *, cases h8 with a h8,
-cases h8 with h8l h8r, specialize h3 a h8l, 
-subst h8r, exact h3,
-specialize h6 h7 h5,
+cases h8 with h8l h8r,
+subst h8r, exact h3 a h8l,
+specialize h6 xΓ.2 h7 h5,
 have h8 := (six xΓ.1 (max_imp_ax xΓ.2)).mp xΓ.2 (K a (¬φ)),
-cases h8 with h8l h8r, simp at *, specialize h8r h6, 
-exact absurd h1 h8r,
+cases h8 with h8l h8r, simp at *, 
+exact absurd h1 (h8r h6),
 },
 have h2 := lindenbaum (Γbox ∪ {φ}) h1,
 cases h2 with Δ h2, cases h2 with h2 h3,
@@ -51,15 +63,12 @@ intros ψ h4, apply h5_left, exact h4,
 exact h3,
 simp at *,
 intros yΔ h1 h2,
-have h3 := h2 φ, 
 by_contradiction h4,
 have h5 := (max_notiff xΓ.1 xΓ.2 (C a φ)).mp h4,
 have h6 := (max_dn xΓ.1 xΓ.2 (K a ¬φ)).mpr h5,
-have h7 := h2 (¬φ), specialize h7 h6,
-simp at *,
-have h8 := (max_notiff yΔ.1 yΔ.2 φ).mpr h7,
-exact absurd h1 h8
+exact absurd h1 ((max_notiff yΔ.1 yΔ.2 φ).mpr ((h2 (¬φ)) h6))
 end
+
 
 lemma truth (hax : sem_cons (∅ : ctx agents) equiv_class) (xΓ : canonical.states) : 
   ∀ φ : form agents, forces canonical val_canonical xΓ φ ↔ (φ ∈ xΓ.val) :=
@@ -69,145 +78,107 @@ intro φ, induction φ with n φ ψ ih_φ ih_ψ
 split, intro h1, exact false.elim h1,
 intro h1, rw forces, 
 have h2 := xΓ.2,
-rw max_ax_consist at h2, cases h2,
-rw ax_consist at h2_left, specialize h2_left [⊥],
-simp at *, specialize h2_left h1, 
-rw fin_ax_consist at h2_left,
-repeat {rw fin_conj at h2_left},
-exact absurd not_contra h2_left,
+cases h2,
+specialize h2_left [⊥],
+simp at *, 
+exact absurd not_contra (h2_left h1),
 repeat {rw forces, rw val_canonical},
 split, intro h1, cases h1 with h1 h2,
-specialize ih_φ xΓ, cases ih_φ,
-specialize ih_ψ xΓ,
-specialize ih_φ_mp h1, cases ih_ψ,
-specialize ih_ψ_mp h2, 
-exact max_conj_1 xΓ.2 (and.intro ih_φ_mp ih_ψ_mp), 
+exact max_conj_1 xΓ.2 (and.intro ((ih_φ xΓ).mp h1) ((ih_ψ xΓ).mp h2)), 
 intro h1, split,
-specialize ih_φ xΓ, cases ih_φ, 
-apply ih_φ_mpr, exact max_conj_2 xΓ.2 h1,
-specialize ih_ψ xΓ, cases ih_ψ, 
-apply ih_ψ_mpr, exact max_conj_3 xΓ.2 h1,
+apply (ih_φ xΓ).mpr, exact max_conj_2 xΓ.2 h1,
+apply (ih_ψ xΓ).mpr, exact max_conj_3 xΓ.2 h1,
 split, 
-intro h1, specialize ih_φ xΓ,
-specialize ih_ψ xΓ, cases ih_φ, cases ih_ψ,
+intro h1,
 apply max_imp_1 xΓ.2,
-intro h2, specialize ih_φ_mpr h2,
-specialize h1 ih_φ_mpr, exact ih_ψ_mp h1,
+intro h2,
+exact (ih_ψ xΓ).mp (h1 ((ih_φ xΓ).mpr h2)),
 intros h1 h2,
-specialize ih_φ xΓ, cases ih_φ,
-specialize ih_ψ xΓ, cases ih_ψ,
-apply ih_ψ_mpr, specialize ih_φ_mp h2,
-exact max_imp_2 xΓ.2 h1 ih_φ_mp,
-split, 
+apply (ih_ψ xΓ).mpr, 
+exact max_imp_2 xΓ.2 h1 ((ih_φ xΓ).mp h2),
 rename φ a, rename ih_φ φ,
+split, 
 intros h1, by_contradiction h2,
-have h4 : C a (¬φ) ∈ xΓ.val → ∃ yΔ : canonical.states, 
-  (¬φ) ∈ yΔ.val ∧ canonical.rel _ xΓ yΔ,
-from (existence hax xΓ a (¬φ)).mp,
+have h4 := (existence hax xΓ a (¬φ)).mp,
 have h5 := max_boxdn xΓ.1 xΓ.2 φ a ((max_notiff xΓ.1 xΓ.2 (K a φ)).mp h2),
-simp at *,
-specialize h4 h5, cases h4 with xΔ h4, cases h4 with h4 h6,
+cases h4 h5 with xΔ h4, cases h4 with h4 h6,
 have h7 := max_notiff xΔ.1 xΔ.2 φ,
 cases h7 with h7l h7r,
-specialize h7r h4, clear h7l h4 h5 h2,
-specialize φ_ih xΔ, specialize h1 xΔ h6,
-cases φ_ih, specialize φ_ih_mp h1,
-exact absurd φ_ih_mp h7r,
-rename φ a, rename ih_φ φ,
+exact absurd ((φ_ih xΔ).mp (h1 xΔ h6)) (h7r h4),
 intros h1 xΔ h2,
-have h3 := h2 φ h1,
-specialize φ_ih xΔ, cases φ_ih, 
-apply φ_ih_mpr, exact h3,
+apply (φ_ih xΔ).mpr, exact (h2 φ h1),
 end
+
 
 lemma comphelper (φ : form agents) (hax : sem_cons (∅ : ctx agents) equiv_class) : 
   ¬ prfS5 ∅ φ → ax_consist ({¬φ} : ctx agents) :=
 begin
-intro h1, rw ax_consist, intros L h2,
-rw fin_ax_consist, induction L, rw fin_conj, 
+intros h1 L h2,
+rw fin_ax_consist, induction L,
 by_contradiction h3,
 exact absurd (mp dne h3) (nprfalse hax), 
 have h4 : (∀ ψ ∈ L_hd::L_tl, ψ = ¬φ) → prfS5 ∅ (¬fin_conj (L_hd::L_tl)) → prfS5 ∅ φ, 
 from fin_conj_repeat hax,
 simp at *, 
 cases h2 with h2 h3,
-specialize h4 h2, intro h6, apply h1, apply h4, 
+intro h6, apply h1, apply h4 h2, 
 exact h3,
 exact h6
 end 
 
+
 theorem forcesAX (hax : sem_cons (∅ : ctx agents) equiv_class) : 
   forces_ctx canonical val_canonical (∅ : ctx agents) :=
 begin
-rw forces_ctx,
 intros φ xΓ h1,
-have h2 : prfS5 ∅ (form.impl (¬form.bot) φ), from mp prfS5.pl1 (ax h1),
+have h2 := mp prfS5.pl1 (ax h1),
 have h3 : ∀ ψ ∈ list.nil, ψ ∈ xΓ.val, 
 {intros ψ h3, have h5 := list.ne_nil_of_length_pos (list.length_pos_of_mem h3),
 simp at *, exact false.elim h5},
-have h4 : φ ∈ xΓ.val, from exercise1 xΓ.2 h3 h2,
+have h4 := exercise1 xΓ.2 h3 h2,
 exact (truth hax xΓ φ).mpr h4
 end
+
 
 lemma euclid_dual {a : agents} {φ : form agents} : 
   prfS5 ∅ ((C a (¬φ) ⊃ K a (C a (¬φ))) ⊃ (C a (K a φ) ⊃ K a φ)) :=
 begin
-simp,
-have h1 : prfS5 ∅ (C a (¬φ) ⊃ K a (C a ¬φ)), from negintro,
-simp at *,
-have h2 : prfS5 ∅ ((¬K a (C a ¬φ)) ⊃ ¬(C a ¬φ)), from contrapos.mpr h1,
-have h3 : prfS5 ∅ ((¬K a (C a ¬φ)) ⊃ (K a φ)), from cut h2 (mp pl6 dual_equiv1),
-have h4 : prfS5 ∅ ((¬K a (C a ¬φ)) ↔ (¬¬C a (¬(C a ¬φ)))),
+have h1 := contrapos.mpr negintro,
+have h2 := cut h1 (mp pl6 dual_equiv1),
+have h3 : prfS5 ∅ ((¬K a (C a ¬φ)) ↔ (¬¬C a (¬(C a ¬φ)))),
   from (mp (mp pl4 (contrapos.mpr (mp pl6 dual_equiv1))) 
   (contrapos.mpr (mp pl5 dual_equiv1))),
-have h5 : prfS5 ∅ (C a (¬(C a ¬φ)) ⊃ (K a φ)), from cut dni (cut (mp pl6 h4) h3),
-have h6 : prfS5 ∅ ((C a (K a φ)) ⊃ (C a (¬(C a ¬φ)))), 
-  from (contrapos.mpr (mp kdist (nec (contrapos.mpr (mp pl5 dual_equiv1))))),
-exact (mp pl1 (cut h6 h5))
+have h4 := cut dni (cut (mp pl6 h3) h2),
+have h5 := (contrapos.mpr (mp kdist (nec (contrapos.mpr (mp pl5 dual_equiv1))))),
+exact (mp pl1 (cut h5 h4))
 end
+
 
 lemma S5_equiv (hax : sem_cons (∅ : ctx agents) equiv_class) : 
   canonical ∈ (equiv_class : set (frame agents)) :=
 begin
 rw equiv_ref_euclid,
 split,
-rw ref_class, rw set.mem_set_of_eq,
-intro a,
-rw reflexive,
-intros x φ h1,
+intros a x φ h1,
 have h2 : ∀ a, (∀ ψ ∈ [(K a φ)], ψ ∈ x.1) → prfS5 ∅ (fin_conj [(K a φ)] ⊃ φ) → φ ∈ x.1, 
   from λ a, exercise1 x.2,
 have h3 : prfS5 ∅ (fin_conj [(K a φ)] ⊃ φ), 
-{repeat {rw fin_conj},
-have h4 : prfS5 ∅ ((K a φ) ⊃ φ), from prfS5.truth,
-exact cut (mp pl5 phi_and_true) h4},
+{exact cut (mp pl5 phi_and_true) prfS5.truth},
 specialize h2 a, simp at *,
 exact h2 h1 h3,
-rw euclid_class,
-rw set.mem_set_of_eq,
-intro a,
-rw euclidean,
-intros x y z h1 h2 φ h3,
-specialize h2 φ,
-apply h2, clear h2,
-have h2 : prfS5 ∅ (C a (¬φ) ⊃ K a (C a ¬φ)), from negintro,
-have h4 : prfS5 ∅ (C a (K a φ) ⊃ K a φ), 
-  from mp euclid_dual h2,
+intros a x y z h1 h2 φ h3,
+apply h2 φ,
+have h4 := mp euclid_dual negintro,
 have h5 : ∀ a, (∀ ψ ∈ [(C a (K a φ))], ψ ∈ x.1) → 
   prfS5 ∅ (fin_conj [(C a (K a φ))] ⊃ K a φ) → K a φ ∈ x.1,
   from λ a, exercise1 x.2, 
 simp at *,
 apply h5,
 by_contradiction h6,
-have h7 : (¬K a (¬K a φ)) ∉ x.1 ↔ (¬(¬K a (¬K a φ))) ∈ x.1, 
-  from max_notiff x.1 x.2 (¬K a (¬K a φ)),
-cases h7, simp at *, specialize h7_mp h6,
-have h8 : (K a (¬K a φ)) ∈ x.1 ↔ (¬¬(K a (¬K a φ))) ∈ x.1, 
-  from max_dn x.1 x.2 (K a (¬K a φ)),
-cases h8, simp at *, specialize h8_mpr h7_mp,
-specialize h1 (¬K a φ) h8_mpr,
-have h9 := (max_notiff y.1 y.2 (K a φ)).mpr h1,
-simp at *, exact absurd h3 h9,
+have h7 := max_notiff x.1 x.2 (¬K a (¬K a φ)),
+have h8 := max_dn x.1 x.2 (K a (¬K a φ)),
+have h9 := (max_notiff y.1 y.2 (K a φ)).mpr (h1 (¬K a φ) (h8.mpr (h7.mp h6))),
+exact absurd h3 h9,
 exact (cut (mp pl5 phi_and_true) h4)
 end
 
@@ -216,8 +187,8 @@ theorem completeness (hax : sem_cons (∅ : ctx agents) equiv_class) (φ : form 
   global_sem_csq ∅ equiv_class φ → prfS5 ∅ φ :=
 begin
 rw ←not_imp_not, intro h1,
-have h2 : ax_consist {¬φ}, from comphelper φ hax h1,
-have h3 : ∃ Γ', max_ax_consist Γ' ∧ {¬φ} ⊆ Γ', from lindenbaum {¬φ} h2,
+have h2 := comphelper φ hax h1,
+have h3 := lindenbaum {¬φ} h2,
 simp at *,
 cases h3 with Γ' h3, cases h3 with h3 h4, 
 rw global_sem_csq, 
@@ -237,7 +208,8 @@ have h5 : forces f v xΓ' (¬φ) ↔ ((¬φ) ∈ xΓ'.val),
 cases h5 with h5 h6,
 have h7 : ¬forces f v xΓ' φ ↔ forces f v xΓ' ¬φ, 
   from not_forces_imp f v xΓ' φ,
-cases h7 with h7 h8, apply h8, apply h6, simp at *, exact h4
+cases h7 with h7 h8, apply h8, apply h6, exact h4
 end
+
 
 end canonical
