src/del/semantics/complexitylemmas.lean
@@ -1,10 +1,18 @@
--- Following the textbook "Dynamic Epistemic Logic" by 
--- Hans van Ditmarsch, Wiebe van der Hoek, and Barteld Kooi
+/-
+Copyright (c) 2021 Paula Neeley. All rights reserved.
+Author: Paula Neeley
+Following the textbook "Dynamic Epistemic Logic" by 
+Hans van Ditmarsch, Wiebe van der Hoek, and Barteld Kooi
+-/
 
 import del.semantics.translationdefs tactic.linarith
+
 variables {agents : Type}
 
+
 ---------------------- Generic helper lemmas ----------------------
+
+
 lemma comp_gt_zero {φ : formPA agents} : complexity φ > 0 :=
 begin
 induction φ,
@@ -13,7 +21,9 @@ have h1 : 4 > 0, linarith,
 exact (mul_pos (add_lt_add h1 φ_ih_φ) φ_ih_ψ)
 end
 
+
 lemma comp_ge_zero {φ : formPA agents} : complexity φ ≥ 0 := le_of_lt comp_gt_zero
+
 
 lemma comp_ge_one {φ : formPA agents} : complexity φ ≥ 1 :=
 begin
@@ -21,11 +31,13 @@ have h1 : complexity φ > 0, from comp_gt_zero,
 linarith
 end
 
+
 lemma maxhelper {n1 n2 n3 n4 : nat} : n1 + n2 < n4 → n1 + n3 < n4 → n1 + max n2 n3 < n4 :=
 begin
 intros h1 h2,
 exact nat.add_lt_of_lt_sub_left (max_lt (nat.lt_sub_left_of_add_lt h1) (nat.lt_sub_left_of_add_lt h2))
 end
+
 
 lemma le_maxhelper {n1 n2 n3 n4 : nat} : n1 + n2 ≤ n4 → n1 + n3 ≤ n4 → n1 + max n2 n3 ≤ n4 :=
 begin
@@ -33,11 +45,12 @@ intros h1 h2,
 have h3 := max_le (nat.le_sub_left_of_add_le h1) (nat.le_sub_left_of_add_le h2),
 rw nat.le_sub_right_iff_add_le at h3,
 have h4 : max n2 n3 + n1 = n1 + max n2 n3, linarith,
-have h5 : n1 + max n2 n3 ≤ n4, from eq.subst h4 h3,
-exact h5, linarith
+exact eq.subst h4 h3, linarith
 end
 
+
 -------------- Helper lemmas for translation function --------------
+
 
 lemma tr1 : ∀ φ ψ : formPA agents, complexity φ < 1 + max (complexity φ) (complexity ψ) := 
 begin
@@ -47,6 +60,7 @@ have h2 := add_comm _ _,
 exact (eq.subst h2 (lt_of_le_of_lt (le_max_left (complexity φ) (complexity ψ)) h1))
 end
 
+
 lemma tr2 : ∀ φ ψ : formPA agents, complexity ψ < 1 + max (complexity φ) (complexity ψ) :=
 begin
 intros φ ψ, 
@@ -55,18 +69,19 @@ have h2 := add_comm _ _,
 exact (eq.subst h2 (lt_of_le_of_lt (le_max_right (complexity φ) (complexity ψ)) h1))
 end
 
+
 lemma tr3 : ∀ φ : formPA agents, 1 + max (complexity φ) 1 < 4 + complexity φ :=
 begin
 intro φ,
 have h1 : complexity φ < complexity φ + 1, from lt_add_one _,
-have h2 : 0 < 2 ↔ 2 ≠ 0, from zero_lt_iff_ne_zero,
-cases h2, 
-specialize h2_mpr (nat.add_one_ne_zero 1),
+have h2 := zero_lt_iff_ne_zero,
 have h3 : 3 + (complexity φ + 1) = complexity φ + 4, from add_comm _ _,
-have h4 : complexity φ + 4 = 4 + complexity φ, from add_comm (complexity φ) 4,
-have h5 : 3 + (complexity φ + 1) = 4 + complexity φ, from (rfl.congr h4).mp h3,
-exact (eq.subst h5 (add_lt_add (lt_add_of_pos_right 1 h2_mpr) (max_lt h1 (lt_add_of_pos_left 1 comp_gt_zero))))
+have h4 := add_comm (complexity φ) 4,
+have h5 := (rfl.congr h4).mp h3,
+exact (eq.subst h5 (add_lt_add (lt_add_of_pos_right 1 (h2.mpr (nat.add_one_ne_zero 1))) 
+  (max_lt h1 (lt_add_of_pos_left 1 comp_gt_zero))))
 end
+
 
 lemma tr4helper {φ ψ : formPA agents} : (4 + complexity φ) * (1 + max (complexity ψ) 1) > 9 :=
 begin
@@ -77,9 +92,9 @@ have h4 := max_eq_left h3,
 have h5 : 1 + max (complexity ψ) 1 ≥ 1 + 1, linarith,
 have h6 : 0 ≤ 2, linarith,
 have h7 : 0 ≤ 4 + complexity φ, linarith,
-have h8 := mul_le_mul h2 h5 h6 h7,
-exact h8,
+exact (mul_le_mul h2 h5 h6 h7),
 end
+
 
 lemma tr4helper1 {n m : nat} : n ≥ 4 → m ≥ 1 → 2 + n * m < n * (1 + m) :=
 begin
@@ -88,20 +103,25 @@ begin
   linarith,
 end
 
-lemma tr4helper2 {φ ψ : formPA agents} : 1 + 1 + (4 + complexity φ) * complexity ψ < (4 + complexity φ) * (1 + complexity ψ) :=
+
+lemma tr4helper2 {φ ψ : formPA agents} : 1 + 1 + (4 + complexity φ) * complexity ψ < 
+  (4 + complexity φ) * (1 + complexity ψ) :=
 begin
 have h1 : 4 + complexity φ ≥ 4, linarith,
 exact (tr4helper1 h1 (comp_ge_one))
 end
 
-lemma tr4helper3 {φ ψ : formPA agents} : 1 + 1 + ((4 + complexity φ) * complexity ψ) < (4 + complexity φ) * (1 + max (complexity ψ) 1) :=
+
+lemma tr4helper3 {φ ψ : formPA agents} : 1 + 1 + ((4 + complexity φ) * complexity ψ) < 
+  (4 + complexity φ) * (1 + max (complexity ψ) 1) :=
 begin
 have h1 : complexity ψ ≥ 1, from comp_ge_one,
 have h2 := max_eq_left h1,
-have h3 : (4 + complexity φ) * (1 + complexity ψ) = (4 + complexity φ) * (1 + max (complexity ψ) 1), 
-from congr_arg (has_mul.mul (4 + complexity φ)) (congr_arg (has_add.add 1) (eq.symm (max_eq_left comp_ge_one))),
+have h3 := congr_arg (has_mul.mul (4 + complexity φ)) (congr_arg (has_add.add 1) 
+  (eq.symm (max_eq_left comp_ge_one))),
 exact (eq.subst h3 tr4helper2)
 end
+
 
 lemma tr4 : ∀ φ ψ : formPA agents, 1 + max (complexity φ) (1 + max ((4 + complexity φ) 
   * complexity ψ) 1) < (4 + complexity φ) * (1 + max (complexity ψ) 1) :=
@@ -113,7 +133,7 @@ have h3 : 1 > 0, linarith,
 have h4 : 4 ≥ 0, linarith,
 have h5 : complexity ψ ≥ 1, from comp_ge_one,
 have h6 : 1 ≥ 1, linarith,
-have h7 : max (complexity ψ) 1 ≥ 1, exact le_max_right (complexity ψ) 1,
+have h7 := le_max_right (complexity ψ) 1,
 have h8 : 3 < 9, linarith,
 have h9 : 1 + 1 + max ((4 + complexity φ) * complexity ψ) 1 = 
   1 + (1 + max ((4 + complexity φ) * complexity ψ) 1), linarith,
@@ -122,11 +142,14 @@ exact (maxhelper (eq.subst (mul_one (1 + complexity φ))
   (eq.subst h9 (maxhelper tr4helper3 (lt_trans h8 tr4helper))))
 end
 
-lemma tr5helper {φ ψ : formPA agents} : 1 + ((4 + complexity φ) * complexity ψ) < (4 + complexity φ) * (1 + (complexity ψ)) :=
+
+lemma tr5helper {φ ψ : formPA agents} : 1 + ((4 + complexity φ) * complexity ψ) < 
+  (4 + complexity φ) * (1 + (complexity ψ)) :=
 begin
 have h1 : 1 + 1 + (4 + complexity φ) * complexity ψ < (4 + complexity φ) * (1 + complexity ψ), from tr4helper2,
 linarith,
 end
+
 
 lemma tr5helper1 {ψ χ : formPA agents} : complexity χ ≤ max (complexity χ) (complexity ψ) :=
 begin
@@ -134,13 +157,16 @@ cases max_choice (complexity ψ) (complexity χ),
 repeat {have h : complexity χ ≤ complexity χ, linarith, exact (le_max_left_of_le h)}
 end
 
-lemma tr5helper2 {ψ χ : formPA agents} : max (complexity ψ) (complexity χ) = complexity ψ → complexity χ ≤ complexity ψ :=
+
+lemma tr5helper2 {ψ χ : formPA agents} : max (complexity ψ) (complexity χ) = complexity ψ → 
+  complexity χ ≤ complexity ψ :=
 begin
 intro h1, 
 have h2 : max (complexity χ) (complexity ψ) = complexity ψ, 
   from eq.substr (max_comm (complexity χ) (complexity ψ)) h1,
 exact (eq.subst h2 tr5helper1)
 end
+
 
 lemma tr5helper3 {φ ψ χ : formPA agents} : complexity χ ≤ complexity ψ → 
   1 + ((4 + complexity φ) * complexity χ) < (4 + complexity φ) * (1 + (complexity ψ)) :=
@@ -152,6 +178,7 @@ have h4 := nat.mul_le_mul_left (4 + complexity φ) h1,
 have h5 : 1 + (4 + complexity φ) * complexity χ ≤ 1 + (4 + complexity φ) * complexity ψ, linarith,
 exact (lt_of_le_of_lt h5 tr5helper)
 end
+
 
 lemma tr5 : ∀ φ ψ χ : formPA agents, 1 + max ((4 + complexity φ) * complexity ψ) 
   ((4 + complexity φ) * complexity χ) < (4 + complexity φ) * (1 + max (complexity ψ) (complexity χ)) :=
@@ -165,6 +192,7 @@ cases max_choice ((4 + complexity φ) * complexity ψ) ((4 + complexity φ) * co
 exact (eq.substr h_1 (eq.substr h (tr5helper3 (tr5helper2 (eq.subst (max_comm (complexity ψ) (complexity χ)) h))))),
 exact (eq.substr h_1 (eq.substr h tr5helper)),
 end
+
 
 lemma tr6 : ∀ φ ψ : formPA agents, 1 + max (complexity φ) (1 + (4 + complexity φ) 
   * complexity ψ) < (4 + complexity φ) * (1 + complexity ψ) :=
@@ -181,6 +209,7 @@ have h8 : 1 + complexity ψ = complexity ψ + 1, linarith,
 exact (maxhelper h6 (eq.subst h8 (eq.subst h7 tr4helper2)))
 end
 
+
 lemma tr7helper1 {φ ψ : formPA agents} : (4 + complexity φ ) * (4 + complexity ψ) 
   = (complexity φ) * (complexity ψ) + 4 * (complexity ψ) + 4 * (complexity φ) + 4 * 4 :=
 begin
@@ -190,6 +219,7 @@ have h3 := add_mul (complexity φ) 4 4,
 linarith
 end
 
+
 lemma tr7helper2 {φ ψ : formPA agents} : 5 + (complexity φ) < (complexity φ) * (complexity ψ) + 4 * (complexity ψ) + 4 * (complexity φ) + 4 * 4 :=
 begin
 have h1 : complexity φ ≥ 1, from comp_ge_one,
@@ -198,11 +228,13 @@ have : complexity φ * complexity ψ ≥ 0, apply nat.zero_le,
 linarith 
 end
 
+
 lemma tr7helper3 {φ ψ : formPA agents} : 5 + (complexity φ) < (4 + complexity φ) * (4 + complexity ψ) :=
 begin
 have h1 := tr7helper1,
 exact (eq.substr h1 tr7helper2)
 end
+
 
 lemma tr7helper4 {φ ψ : formPA agents} : 5 + (complexity φ) * (complexity ψ) + 4 * (complexity ψ) < 
   (complexity φ) * (complexity ψ) + 4 * (complexity ψ) + 4 * (complexity φ) + 4 * 4 :=
@@ -218,6 +250,7 @@ have h5 : 5 + (complexity φ) * (complexity ψ) + 4 * (complexity ψ) <
 exact h5
 end
 
+
 lemma tr7helper5 {φ ψ : formPA agents} : 5 + (complexity φ) * (complexity ψ) + 4 * (complexity ψ) =
   (5 + ((4 + complexity φ) * complexity ψ)) :=
 begin
@@ -227,6 +260,7 @@ have h2 : 5 + (complexity φ) * (complexity ψ) + 4 * (complexity ψ)
 exact h2
 end
 
+
 lemma tr7helper6 {φ ψ : formPA agents} : (5 + ((4 + complexity φ) * complexity ψ)) 
   < (4 + complexity φ) * (4 + complexity ψ) :=
 begin
@@ -234,6 +268,7 @@ have h1 := tr7helper5,
 have h2 := tr7helper1,
 exact (eq.substr h2 (eq.subst h1 tr7helper4))
 end
+
 
 lemma tr7 : ∀ φ ψ χ : formPA agents, (4 + (1 + max (complexity φ) ((4 + complexity φ) 
   * complexity ψ))) * complexity χ < (4 + complexity φ) * ((4 + complexity ψ) * complexity χ) :=
@@ -259,6 +294,7 @@ begin
   linarith
 end
 
+
 lemma compand2 {φ ψ : formPA agents} {n : nat} : complexity (φ & ψ) ≤ n + 1 → complexity ψ ≤ n :=
 begin
   intro h,
@@ -266,6 +302,7 @@ begin
   have h1 := le_max_right (complexity φ) (complexity ψ),
   linarith
 end
+
 
 lemma compimp1 {φ ψ : formPA agents} {n : nat} : complexity (φ ⊃ ψ) ≤ n + 1 → complexity φ ≤ n :=
 begin
@@ -275,6 +312,7 @@ begin
   linarith
 end
 
+
 lemma compimp2 {φ ψ : formPA agents} {n : nat} : complexity (φ ⊃ ψ) ≤ n + 1 → complexity ψ ≤ n :=
 begin
   intro h,
@@ -283,10 +321,10 @@ begin
   linarith
 end
 
+
 lemma updatecomphelper {φ ψ : formPA agents} : 
   complexity (U φ ψ) = (complexity φ + 4) * complexity ψ :=
 begin
-rw complexity,
 have h1 := add_comm 4 (complexity φ),
 have h2 : (4 + complexity φ) * complexity ψ = (4 + complexity φ) * complexity ψ, refl,
 exact (eq.subst h1 h2),
@@ -308,6 +346,7 @@ have h7 : (4 + complexity φ) * (complexity ψ) <
 linarith
 end
 
+
 lemma updatecompand2 {φ ψ χ : formPA agents} {n : nat} : 
   complexity (U φ (ψ & χ)) ≤ n + 1 → complexity (U φ χ) ≤ n :=
 begin
@@ -322,6 +361,7 @@ have h7 : (4 + complexity φ) * (complexity ψ) <
   (4 + complexity φ) + (4 + complexity φ) * (complexity ψ), linarith,
 linarith
 end
+
 
 lemma updatecompimp1 {φ ψ χ : formPA agents} {n : nat} : 
   complexity (U φ (ψ ⊃ χ)) ≤ n + 1 → complexity (U φ ψ) ≤ n :=
@@ -338,6 +378,7 @@ have h7 : (4 + complexity φ) * (complexity ψ) <
 linarith
 end
 
+
 lemma updatecompimp2 {φ ψ χ : formPA agents} {n : nat} : 
   complexity (U φ (ψ ⊃ χ)) ≤ n + 1 → complexity (U φ χ) ≤ n :=
 begin
@@ -352,6 +393,7 @@ have h7 : (4 + complexity φ) * (complexity ψ) <
   (4 + complexity φ) + (4 + complexity φ) * (complexity ψ), linarith,
 linarith
 end
+
 
 lemma updatecompknow1' (φ ψ : formPA agents) {n : nat} {a : agents} : complexity (U φ (K a ψ)) ≤ n + 1 
   → 1 + complexity φ ≤ n :=
@@ -374,6 +416,7 @@ have h11 : 1 + complexity φ ≤
   complexity φ * complexity ψ + complexity φ * 1 + 4 * complexity ψ, linarith,
 exact le_trans h11 h10
 end 
+
 
 lemma updatecompknow2' {φ ψ : formPA agents} {n : nat} : (4 + complexity φ) * (1 + complexity ψ) ≤ n + 1 
   → 1 + (1 + (4 + complexity φ) * complexity ψ) ≤ n :=
@@ -408,40 +451,34 @@ have h17 : 1 + (1 + (4 + complexity φ) * complexity ψ) ≤
 exact le_trans h17 h10
 end
 
+
 lemma updatecompknow1 {a : agents} {φ ψ : formPA agents} {n : nat} : 
   complexity (U φ (K a ψ)) ≤ n + 1 → complexity φ ≤ n :=
 begin
 intro h1,
-have h2 : 1 + complexity φ ≤ n, from updatecompknow1' φ ψ h1,
+have h2 := updatecompknow1' φ ψ h1,
 linarith
 end
+
 
 lemma updatecompknow2 {a : agents} {φ ψ : formPA agents} {n : nat} : 
   complexity (U φ (K a ψ)) ≤ n + 1 → complexity (φ ⊃ K a (U φ ψ)) ≤ n :=
 begin
 intro h1,
-have h2 : 1 + complexity φ ≤ n, from updatecompknow1' φ ψ h1,
-have h3 : 1 + (1 + (4 + complexity φ) * complexity ψ) ≤ n, from updatecompknow2' h1,
-have h4 : 1 + max (complexity φ) (1 + (4 + complexity φ) * complexity ψ) ≤ n, from le_maxhelper h2 h3,
-exact h4
+exact le_maxhelper (updatecompknow1' φ ψ h1) (updatecompknow2' h1)
 end
  
+
 lemma updatecompupdate {φ ψ χ : formPA agents} {n : nat} : 
   complexity (U φ (U ψ χ)) ≤ n + 1 → complexity (U (φ & U φ ψ) χ) ≤ n :=
 begin
 intro h1, repeat {rw complexity at *},
-have h2 := tr7 φ ψ χ,
-have h3 := add_left_comm 1 4 (max (complexity φ) ((complexity φ + 4) * complexity ψ)),
-have h5 : (1 + (4 + max (complexity φ) ((4 + complexity φ) * complexity ψ))) = 
+have h2 := add_left_comm 1 4 (max (complexity φ) ((complexity φ + 4) * complexity ψ)),
+have h3 : (1 + (4 + max (complexity φ) ((4 + complexity φ) * complexity ψ))) = 
   (4 + (1 + max (complexity φ) ((4 + complexity φ) * complexity ψ))), 
-  from eq.subst (add_comm (complexity φ) 4) h3,
-have h6 : (1 + (4 + max (complexity φ) ((4 + complexity φ) * complexity ψ))) * complexity χ = 
+  from eq.subst (add_comm (complexity φ) 4) h2,
+have h4 : (1 + (4 + max (complexity φ) ((4 + complexity φ) * complexity ψ))) * complexity χ = 
   (1 + (4 + max (complexity φ) ((4 + complexity φ) * complexity ψ))) * complexity χ, refl,
-have h7 : (1 + (4 + max (complexity φ) ((4 + complexity φ) * complexity ψ))) * complexity χ =
-  (4 + (1 + max (complexity φ) ((4 + complexity φ) * complexity ψ))) * complexity χ, 
-  from eq.subst h5 h6,
-have h8 := add_comm 4 (complexity φ),
-have h9 : complexity (U φ ψ) = (complexity φ + 4) * complexity ψ, from updatecomphelper,
-have h10 := lt_of_lt_of_le h2 h1,
-linarith,
+have h5 := lt_of_lt_of_le (tr7 φ ψ χ) h1,
+linarith
 end
