src/del/semantics/semanticsDEL.lean
@@ -1,23 +1,28 @@
--- Following the textbook "Dynamic Epistemic Logic" by 
--- Hans van Ditmarsch, Wiebe van der Hoek, and Barteld Kooi
+/-
+Copyright (c) 2021 Paula Neeley. All rights reserved.
+Author: Paula Neeley
+Following the textbook "Dynamic Epistemic Logic" by 
+Hans van Ditmarsch, Wiebe van der Hoek, and Barteld Kooi
+-/
+
 
 import del.languageDEL del.syntax.syntaxDEL data.set.basic
 import del.semantics.translationfunction
+local attribute [instance] classical.prop_decidable
 
+variable {agents : Type}
 open formPA 
 open form
 open set
-local attribute [instance] classical.prop_decidable
 
 
 ---------------------- Semantics ----------------------
-
-variable {agents : Type}
 
 structure frame (agents : Type) :=
 (states : Type)
 (h : nonempty states)
 (rel : agents → states → states → Prop)
+
 
 def frame.restrict (f : frame agents) (P : f.states → Prop) (s : f.states) (Ps : P s) : frame agents :=
 {
@@ -26,16 +31,17 @@ def frame.restrict (f : frame agents) (P : f.states → Prop) (s : f.states) (Ps
   rel := λ a : agents, λ u v, f.rel a u.val v.val
 }
 
+
 variables {α : Type} 
 variables (r : α → α → Prop)
 
-def euclidean := ∀ ⦃x y z⦄, r x y → r x z → r y z 
-def euclid_class : set (frame agents ) := { f : frame agents | ∀ a : agents, euclidean (f.rel a) }
-def ref_class : set (frame agents) := { f : frame agents | ∀ a : agents, reflexive (f.rel a) }
-def equiv_class : set (frame agents) := { f : frame agents | ∀ a : agents, equivalence (f.rel a) }
+def euclidean    := ∀ ⦃x y z⦄, r x y → r x z → r y z 
+def euclid_class : set (frame agents ) := { f : frame agents | ∀ a : agents, euclidean   (f.rel a) }
+def ref_class    : set (frame agents)  := { f : frame agents | ∀ a : agents, reflexive   (f.rel a) }
+def equiv_class  : set (frame agents)  := { f : frame agents | ∀ a : agents, equivalence (f.rel a) }
 
 
--- definition of forces for public announcement logic
+-- Definition of forces for public announcement logic
 def forcesPA : ∀ f : frame agents, 
   (nat → f.states → Prop) → f.states → formPA agents → Prop
   | f v x bot          := false
@@ -52,18 +58,22 @@ def m_validPA (φ : formPA agents) (f : frame agents)
   (v : nat → f.states → Prop) := 
   ∀ x, forcesPA f v x φ
 
--- valid in a frame f
+
+-- Valid in a frame f
 def f_validPA (φ : formPA agents) (f : frame agents) := 
   ∀ v x, forcesPA f v x φ
+
 
 -- φ is valid in a class of frames F
 def F_validPA (φ : formPA agents) (F : set (frame agents)) := 
   ∀ f ∈ F, ∀ v x, forcesPA f v x φ
 
+
 -- A context is true at a world in a model if each 
 -- formula of the context is true at that world in that model
 def forces_ctxPA (f : frame agents) (v : nat → f.states → Prop) 
   (Γ : ctxPA agents) := ∀ φ, ∀ x, φ ∈ Γ → forcesPA f v x φ
+
 
 -- Global semantic consequence
 def global_sem_csqPA (Γ : ctxPA agents) (F : set (frame agents)) (φ : formPA agents) :=
@@ -74,16 +84,17 @@ lemma not_forces_impPA (f : frame agents) : ∀ v x φ,
   (¬(forcesPA f v x φ)) ↔ (forcesPA f v x (¬φ)) :=
 begin
 intros v x φ, split, 
-{intros h1 h2, exact h1 h2},
-{intros h1 h2, specialize h1 h2, exact h1}
+repeat {intros h1 h2, exact h1 h2},
 end
 
-lemma forces_existsPA {a : agents} {f : frame agents} {v : nat → f.states → Prop} {x : f.states} {φ : formPA agents} :
+
+lemma forces_existsPA {a : agents} {f : frame agents} {v : nat → f.states → Prop} 
+  {x : f.states} {φ : formPA agents} :
   forcesPA f v x (¬K a ¬φ) ↔ ∃ y : f.states, (f.rel a x y ∧ forcesPA f v y φ) :=
 begin
 split,
 intro h1,
-rw forcesPA at h1, rw forcesPA at h1,
+repeat {rw forcesPA at h1},
 have h2 := not_or_of_imp h1,
 clear h1, cases h2, push_neg at h2,
 cases h2 with y h2, cases h2 with h2 h3,
@@ -91,36 +102,38 @@ existsi (y : f.states), split, exact h2,
 have h4 := (not_forces_impPA f v y (¬φ)).mp h3,
 repeat {rw forcesPA at h4}, repeat {rw imp_false at h4},
 rw not_not at h4, exact h4,
-rw forcesPA at h2, exact false.elim h2,
+exact false.elim h2,
 intro h1, cases h1 with y h1,
 cases h1 with h1 h2,
-rw forcesPA,
 intro h3,
-rw forcesPA at h3, specialize h3 y h1,
+specialize h3 y h1,
 rw ←not_forces_impPA at h3, 
 exact absurd h2 h3
 end
 
-lemma forces_update_dual (φ ψ : formPA agents) (f : frame agents) (v : nat → f.states → Prop) (x : f.states) : 
-forcesPA f v x ¬(U φ (¬ψ)) ↔ ∃ h : forcesPA f v x φ, 
-      forcesPA (f.restrict (λ y, forcesPA f v y φ) x h) (λ n u, v n u.val) ⟨x, h⟩ ψ :=
+
+lemma forces_update_dual (φ ψ : formPA agents) (f : frame agents) 
+  (v : nat → f.states → Prop) (x : f.states) :
+  forcesPA f v x ¬(U φ (¬ψ)) ↔ ∃ h : forcesPA f v x φ, 
+  forcesPA (f.restrict (λ y, forcesPA f v y φ) x h) (λ n u, v n u.val) ⟨x, h⟩ ψ :=
 begin
 split,
-{intro h1, rw forcesPA at h1, rw forcesPA at h1,
-rw forcesPA at h1, rw imp_false at h1,
+{intro h1, repeat {rw forcesPA at h1},
+rw imp_false at h1,
 push_neg at h1,
 cases h1 with Ph1 h1, 
-existsi (Ph1 : forcesPA f v x φ), rw not_forces_impPA at h1, 
-rw forcesPA at h1, rw forcesPA at h1,
-rw forcesPA at h1, rw imp_false at h1, 
+existsi (Ph1 : forcesPA f v x φ), 
+rw not_forces_impPA at h1, 
+repeat {rw forcesPA at h1}, 
+rw imp_false at h1, 
 push_neg at h1,
 cases h1 with Ph2 h2, exact Ph2},
 {intro h1, cases h1 with Ph1 h1, 
 intro h2, apply h2, exact h1}
 end
 
--- definition of forces for basic modal language indexed over agents...
--- used for typeclass inference between systems
+
+-- Definition of forces for epistemic logic...used for typeclass inference between systems
 def forces : ∀ f : frame agents, 
   (nat → f.states → Prop) → f.states → form agents → Prop
   | f v x form.bot          := false
@@ -129,85 +142,71 @@ def forces : ∀ f : frame agents,
   | f v x (form.impl φ ψ)   := (forces f v x φ) → (forces f v x ψ)
   | f v x (form.box a φ)    := ∀ y, f.rel a x y → forces f v y φ
 
-lemma forcesPA_iff_forces (φ : form agents) (f : frame agents) : 
-  ∀ v x, forcesPA f v x (to_PA φ) ↔ forces f v x φ :=
-begin
-intros v x, induction φ generalizing x,
-split,
-repeat {intro h1,
-apply h1},
-split,
-repeat {intro h1,
-apply h1},
-rename φ_ih_φ ih_φ,
-rename φ_ih_ψ ih_ψ,
-specialize ih_φ x,
-specialize ih_ψ x,
-cases ih_φ, cases ih_ψ,
-split,
-intro h1,
-cases h1 with h1 h2,
-split,
-exact ih_φ_mp h1,
-exact ih_ψ_mp h2,
-intro h1,
-cases h1 with h1 h2,
-split,
-exact ih_φ_mpr h1,
-exact ih_ψ_mpr h2,
-rename φ_ih_φ ih_φ,
-rename φ_ih_ψ ih_ψ,
-specialize ih_φ x,
-specialize ih_ψ x,
-cases ih_φ, cases ih_ψ,
-split,
-intros h1 h2,
-specialize ih_φ_mpr h2,
-specialize h1 ih_φ_mpr,
-exact ih_ψ_mp h1,
-intros h1 h2,
-specialize ih_φ_mp h2,
-specialize h1 ih_φ_mp,
-exact ih_ψ_mpr h1,
-split,
-intros h1 y h3,
-specialize h1 y h3,
-specialize φ_ih y,
-cases φ_ih,
-exact φ_ih_mp h1,
-intros h1 y h3,
-specialize h1 y h3,
-specialize φ_ih y,
-cases φ_ih,
-exact φ_ih_mpr h1
-end
 
 def F_valid (φ : form agents) (F : set (frame agents)) := 
   ∀ f ∈ F, ∀ v x, forces f v x φ
+
 
 -- A context is true at a world in a model if each 
 -- formula of the context is true at that world in that model
 def forces_ctx (f : frame agents) (v : nat → f.states → Prop) 
   (Γ : ctx agents) := ∀ φ : form agents, ∀ x, φ ∈ Γ → forces f v x φ
 
--- global semantic consequence
+
+-- Global semantic consequence
 def global_sem_csq (Γ : ctx agents) (F : set (frame agents)) (φ : form agents) :=
   ∀ f ∈ F, ∀ v, forces_ctx f v Γ → ∀ x, forces f v x φ
+
+
+lemma forcesPA_iff_forces (φ : form agents) (f : frame agents) : 
+  ∀ v x, forcesPA f v x (to_PA φ) ↔ forces f v x φ :=
+begin
+intros v x, induction φ generalizing x,
+split,
+repeat {intro h1, apply h1},
+split,
+repeat {intro h1, apply h1},
+repeat {rename φ_ih_φ ih_φ},
+repeat {rename φ_ih_ψ ih_ψ},
+split,
+intro h1,
+cases h1 with h1 h2,
+split,
+exact (ih_φ x).mp h1,
+exact (ih_ψ x).mp h2,
+intro h1,
+cases h1 with h1 h2,
+split,
+exact (ih_φ x).mpr h1,
+exact (ih_ψ x).mpr h2,
+split,
+intros h1 h2,
+exact (ih_ψ x).mp (h1 ((ih_φ x).mpr h2)),
+intros h1 h2,
+exact (ih_ψ x).mpr (h1 ((ih_φ x).mp h2)),
+split,
+intros h1 y h3,
+exact (φ_ih y).mp (h1 y h3),
+intros h1 y h3,
+exact (φ_ih y).mpr (h1 y h3)
+end
+
 
 lemma not_forces_imp (f : frame agents) : ∀ v x φ, 
   (¬(forces f v x φ)) ↔ (forces f v x (¬φ)) :=
 begin
 intros v x φ, split, 
-{intros h1 h2, exact h1 h2},
-{intros h1 h2, specialize h1 h2, exact h1}
+repeat {intros h1 h2, exact h1 h2},
 end
 
-lemma forces_exists {a : agents} {f : frame agents} {v : nat → f.states → Prop} {x : f.states} {φ : form agents} :
+
+lemma forces_exists {a : agents} {f : frame agents} {v : nat → f.states → Prop} 
+  {x : f.states} {φ : form agents} :
   forces f v x (¬K a ¬φ) ↔ ∃ y : f.states, (f.rel a x y ∧ forces f v y φ) :=
 begin
 split,
 intro h1,
-rw forces at h1, rw forces at h1,
+repeat {rw forces at h1},
 have h2 := not_or_of_imp h1,
 clear h1, cases h2, push_neg at h2,
 cases h2 with y h2, cases h2 with h2 h3,
@@ -219,35 +218,28 @@ exact false.elim h2,
 intro h1, cases h1 with y h1,
 cases h1 with h1 h2,
 intro h3,
-specialize h3 y h1,
-rw ←not_forces_imp at h3, 
-exact absurd h2 h3
+exact absurd h2 (h3 y h1)
 end
 
+
 lemma equiv_ref_euclid (f : frame agents) : 
-  f ∈ (equiv_class : set (frame agents)) ↔ f ∈ ((ref_class : set (frame agents)) ∩ (euclid_class : set (frame agents))) :=
+  f ∈ (equiv_class : set (frame agents)) ↔ 
+  f ∈ ((ref_class : set (frame agents)) ∩ (euclid_class : set (frame agents))) :=
 begin
-rw equiv_class, rw ref_class, rw euclid_class,
-rw set.mem_set_of_eq, simp, split,
+split,
 intro h1,
 split,
 intro a,
-specialize h1 a,
-cases h1 with h1 h2, cases h2 with h2 h3,
+cases h1 a with h1 h2, cases h2 with h2 h3,
 exact h1,
-intro a, rw euclidean, intros x y z h4 h5,
-specialize h1 a, rw equivalence at h1,
-cases h1 with h1 h2, cases h2 with h2 h3,
-rw symmetric at h2, specialize h2 h4, 
-rw transitive at h3, exact h3 h2 h5,
-intros h1 a, rw equivalence, split,
-cases h1, exact h1_left a,
-split, cases h1 with h1 h2, rw symmetric,
-intros x y h3, specialize h2 a, rw euclidean at h2, 
-specialize h1 a, rw reflexive at h1,
-specialize h1 x, exact h2 h3 h1,
-rw transitive, intros x y z h2 h3, cases h1 with h1 h4,
-specialize h4 a, rw euclidean at h4, specialize h1 a, 
-rw reflexive at h1, specialize h1 x, have h5 := h4 h2 h1, 
-exact h4 h5 h3
+intro a, intros x y z h4 h5,
+cases h1 a with h1 h2, cases h2 with h2 h3,
+exact h3 (h2 h4) h5,
+intros h1 a, split,
+exact h1.left a,
+split, cases h1 with h1 h2,
+intros x y h3,
+exact (h2 a) h3 (h1 a x),
+intros x y z h2 h3, cases h1 with h1 h4,
+exact h4 a (h4 a h2 (h1 a x)) h3
 end
