src/del/semantics/translation.lean
@@ -1,16 +1,20 @@
--- Following the textbook "Dynamic Epistemic Logic" by 
--- Hans van Ditmarsch, Wiebe van der Hoek, and Barteld Kooi
+/-
+Copyright (c) 2021 Paula Neeley. All rights reserved.
+Author: Paula Neeley
+Following the textbook "Dynamic Epistemic Logic" by 
+Hans van Ditmarsch, Wiebe van der Hoek, and Barteld Kooi
+-/
 
 import del.semantics.translationlemmas
 import del.semantics.completenessDEL del.syntax.syntaxlemmasPADEL
 import tactic.linarith
 
 variables {agents : Type}
-
 open prfPA
 open PAlemma
 
 ---------------------- Completeness by Translation ----------------------
+
 
 theorem equiv_translation_aux' {Γ : ctxPA agents} (n : nat) (φ : formPA agents) (h : complexity φ ≤ n) : 
   prfPA Γ (φ ↔ to_PA (translate φ)) :=
@@ -25,22 +29,17 @@ begin
     { exact mp (mp pl4 iden) iden },
   case formPA.and : φ ψ 
     { rw translate,
-      have h1 := ih φ (compand1 h),
-      have h2 := ih ψ (compand2 h),
-      exact iff_iff_and_iff h1 h2
+      exact iff_iff_and_iff (ih φ (compand1 h)) (ih ψ (compand2 h))
     },
   case formPA.impl : φ ψ 
     { rw translate,
       repeat {rw to_PA},
-      have h1 := ih φ (compimp1 h),
-      have h2 := ih ψ (compimp2 h),
-      exact iff_iff_imp_iff h1 h2
+      exact iff_iff_imp_iff (ih φ (compimp1 h)) (ih ψ (compimp2 h))
     },
   case formPA.box : a φ 
     { simp at *,
       have h1 : complexity φ ≤ n, from nat.lt_succ_iff.mp (nat.one_add_le_iff.mp h),
-      have h2 := ih φ h1,
-      exact iff_k_dist h2, 
+      exact iff_k_dist (ih φ h1), 
     },
   case formPA.update : φ ψ 
     { cases ψ,
@@ -50,9 +49,8 @@ begin
           have h1 : complexity φ ≤ n, 
             {have : complexity φ + 1 ≤ nat.succ n, linarith,
              exact nat.lt_succ_iff.mp this},
-          have h2 := ih φ h1,
-          have h3 : prfPA Γ ((U φ ⊥) ↔ (φ ⊃ ⊥)), from atomicbot, 
-          exact update_iff1 h2 h3 
+          have h2 := atomicbot, 
+          exact update_iff1 (ih φ h1) h2
         },
       case formPA.var : m 
         { repeat {rw translate},
@@ -60,37 +58,24 @@ begin
           have h1 : complexity φ ≤ n, 
             {have : complexity φ + 1 ≤ nat.succ n, linarith,
              exact nat.lt_succ_iff.mp this},
-          have h2 := ih φ h1,
-          have h3 : prfPA Γ ((U φ (p m)) ↔ (φ ⊃ (p m))), from atomicperm, 
-          exact update_iff1 h2 h3 
+          have h2 := atomicperm, 
+          exact update_iff1 (ih φ h1) h2
         },
       case formPA.and : ψ χ 
         { repeat {rw translate},
-          have h1 : prfPA Γ ((U φ (ψ & χ)) ↔ ((U φ ψ) & (U φ χ))), from announceconj,
-          have h2 := ih (U φ ψ) (updatecompand1 h),
-          have h3 := ih (U φ χ) (updatecompand2 h),
-          simp at *,
-          exact update_iff2 h2 h3 h1,
+          exact update_iff2 (ih (U φ ψ) (updatecompand1 h)) (ih (U φ χ) (updatecompand2 h)) announceconj,
         },
       case formPA.impl : ψ χ
         { repeat {rw translate},
-          have h1 : prfPA Γ ((U φ (ψ ⊃ χ)) ↔ ((U φ ψ) ⊃ (U φ χ))), from announceimp,
-          have h2 := ih (U φ ψ) (updatecompimp1 h),
-          have h3 := ih (U φ χ) (updatecompimp2 h),
-          simp at *,
-          exact update_iff3 h2 h3 h1,
+          exact update_iff3 (ih (U φ ψ) (updatecompimp1 h)) (ih (U φ χ) (updatecompimp2 h)) announceimp,
         },
       case formPA.box : a ψ
         { repeat {rw translate}, 
-          have h1 : prfPA Γ ((U φ (K a ψ)) ↔ (φ ⊃ (K a (U φ ψ)))), from announceknow,
-          have h2 := ih (φ ⊃ K a (U φ ψ)) (updatecompknow2 h),
-          exact update_iff4 h1 h2
+          exact update_iff4 announceknow (ih (φ ⊃ K a (U φ ψ)) (updatecompknow2 h))
         },
       case formPA.update : ψ χ
-        { rw translate,
-          have h1 : prfPA Γ ((U φ (U ψ χ)) ↔ (U (φ & (U φ ψ)) χ)), from announcecomp,
-          have h2 := ih (U (φ & (U φ ψ)) χ) (updatecompupdate h),
-          exact update_iff5 h1 h2,
+        { rw translate, 
+          exact update_iff5 announcecomp (ih (U (φ & (U φ ψ)) χ) (updatecompupdate h))
         } 
     }
 end
@@ -104,6 +89,7 @@ simp,
 exact equiv_translation_aux' (complexity φ + 1) φ h
 end
 
+
 lemma forces_ctxPA_iff_forces_ctx (f : frame agents) 
   (v : nat → f.states → Prop) : 
   forces_ctxPA f v ∅ ↔ forces_ctx f v ∅ :=
@@ -113,12 +99,12 @@ repeat {intros h1 φ x h2,
 exact false.elim h2},
 end
 
+
 lemma global_sem_csqPA_iff_global_sem_csq (F : set (frame agents)) (φ : form agents) : 
   global_sem_csqPA ∅ F (to_PA φ) ↔ global_sem_csq ∅ F φ :=
 begin
 split,
 intros h1 f h2 v h3 x,
-rw global_sem_csqPA at h1,
 have h4 := (forces_ctxPA_iff_forces_ctx f v).mpr h3,
 exact (forcesPA_iff_forces φ f v x).mp (h1 f h2 v h4 x),
 intros h1 f h2 v h3 x,
@@ -126,28 +112,20 @@ have h4 := (forces_ctxPA_iff_forces_ctx f v).mp h3,
 exact (forcesPA_iff_forces φ f v x).mpr (h1 f h2 v h4 x)
 end
 
+
 theorem completenessPA {φ : formPA agents} (Γ : ctxPA agents) : 
   global_sem_csqPA ∅ equiv_class φ → prfPA ∅ φ :=
 begin
 intros h1,
-have h2 : prfPA ∅ (φ ⊃ to_PA (translate φ)), 
-  from mp pl5 (equiv_translation ∅ φ),
-have h3 : prfPA ∅ (φ ⊃ to_PA (translate φ)) → 
-  global_sem_csqPA ∅ equiv_class (φ ⊃ to_PA (translate φ)), 
-  from soundnessPA,
-specialize h3 h2,
+have h2 := mp pl5 (equiv_translation ∅ φ),
+have h3 := soundnessPA,
 have h4 : global_sem_csqPA ∅ equiv_class (to_PA (translate φ)), 
-{rw global_sem_csqPA, intros f h4 v h5 x,
-specialize h1 f h4 v h5 x, specialize h3 f h4 v h5 x, exact h3 h1},
-have h5 : global_sem_csq (∅ : ctx agents) equiv_class (translate φ), 
-  from (global_sem_csqPA_iff_global_sem_csq equiv_class (translate φ) ).mp h4,
-have h6 : global_sem_csq ∅ equiv_class (translate φ) → prfS5 ∅ (translate φ), 
-  from canonical.completeness sem_consS5 (translate φ),
+{intros f h4 v h5 x,
+exact h3 h2 f h4 v h5 x (h1 f h4 v h5 x)},
+have h5 := (global_sem_csqPA_iff_global_sem_csq equiv_class (translate φ) ).mp h4,
+have h6 := canonical.completeness sem_consS5 (translate φ),
 specialize h6 h5,
-have h7 : prfPA (to_PA '' ∅) (to_PA (translate φ)), from to_prfPA h6,
-have h8 : prfPA ∅ (φ ↔ to_PA (translate φ)), from equiv_translation ∅ φ,
+have h7 := to_prfPA h6,
 simp at *,
-have h9 : prfPA ∅ ((to_PA (translate φ)) ⊃ φ), from mp pl6 h8,
-have h10 : prfPA ∅ φ, from mp h9 h7,
-exact h10
+exact mp (mp pl6 (equiv_translation ∅ φ)) h7
 end
