src/del/syntax/soundnessDEL.lean
@@ -1,13 +1,18 @@
--- Following the textbook "Dynamic Epistemic Logic" by 
--- Hans van Ditmarsch, Wiebe van der Hoek, and Barteld Kooi
+/-
+Copyright (c) 2021 Paula Neeley. All rights reserved.
+Author: Paula Neeley
+Following the textbook "Dynamic Epistemic Logic" by 
+Hans van Ditmarsch, Wiebe van der Hoek, and Barteld Kooi
+-/
 
 import del.languageDEL data.set.basic del.semantics.semanticsDEL del.announcements
-variables {agents : Type}
 local attribute [instance] classical.prop_decidable
 
+variables {agents : Type}
 
 
 ---------------------- Soundness ----------------------
+
 
 theorem soundnessS5 {Γ : ctx agents} {φ : form agents} : 
   prfS5 Γ φ → global_sem_csq Γ equiv_class φ :=
@@ -25,13 +30,12 @@ repeat {rename h1_hpq hpq},
 repeat {rename h1_ih ih},
 repeat {rename h1_ih_hp ih_hp},
 repeat {rename h1_ih_hpq ih_hpq},
-{specialize h3 φ x h1, exact h3},
+{exact h3 φ x h1},
 {intros h4 h5, exact h4},
 {intros h4 h5 h6, exact (h4 h6) (h5 h6)},
 {intros h1 h4,
 by_contradiction h5,
-specialize h4 h5, specialize h1 h5, 
-rw ← not_forces_imp at h1, exact h1 h4},
+exact (h1 h5) (h4 h5)},
 {intros h4 h5, exact and.intro h4 h5}, 
 {intros h4, exact h4.left}, 
 {intros h4, exact h4.right}, 
@@ -45,15 +49,14 @@ rw not_imp_not at h1,
 exact h1 h4}, 
 {intros h3 h4, simp [forces] at *, intros x' h5, 
 exact (h3 x' h5) (h4 x' h5)},
-{intros h1, apply h1, specialize h2 a, exact h2.left x}, 
-{intros h1 y h4 z h5, specialize h1 z, apply h1,
-specialize h2 a, cases h2 with h2l h2r, cases h2r with h2r h2rr,
-specialize h2rr h4 h5, exact h2rr}, 
-{intros h1 y h5 h4, apply h1, intros z h6, specialize h4 z, apply h4, 
-specialize h2 a, cases h2 with h2l h2r, cases h2r with h2r h2rr, 
+{intros h1, apply h1, exact (h2 a).left x}, 
+{intros h1 y h4 z h5, apply h1 z,
+cases h2 a with h2l h2r, cases h2r with h2r h2rr,
+exact h2rr h4 h5}, 
+{intros h1 y h5 h4, apply h1, intros z h6, apply h4 z, 
+cases h2 a with h2l h2r, cases h2r with h2r h2rr, 
 exact h2rr (h2r h5) h6},
-{specialize ih_hp h3 x, specialize ih_hpq h3 x ih_hp, 
-exact ih_hpq},
+{exact ih_hpq h3 x (ih_hp h3 x)},
 {intros y h1, exact ih h3 y} 
 end
 
@@ -74,13 +77,12 @@ repeat {rename h1_hpq hpq},
 repeat {rename h1_ih ih},
 repeat {rename h1_ih_hp ih_hp},
 repeat {rename h1_ih_hpq ih_hpq},
-{specialize h3 φ x h1, exact h3},
+{exact h3 φ x h1},
 {intros h4 h5, exact h4},
 {intros h4 h5 h6, exact (h4 h6) (h5 h6)},
 {intros h1 h4,
 by_contradiction h5,
-specialize h4 h5, specialize h1 h5, 
-rw ← not_forces_impPA at h1, exact h1 h4},
+exact (h1 h5) (h4 h5)},
 {intros h4 h5, exact and.intro h4 h5}, 
 {intros h4, exact h4.left}, 
 {intros h4, exact h4.right}, 
@@ -94,29 +96,26 @@ rw not_imp_not at h1,
 exact h1 h4}, 
 {intros h3 h4, simp [forcesPA] at *, intros x' h5, 
 exact (h3 x' h5) (h4 x' h5)},
-{intros h1, apply h1, specialize h2 a, exact h2.left x}, 
-{intros h1 y h4 z h5, specialize h1 z, apply h1,
-specialize h2 a, cases h2 with h2l h2r, cases h2r with h2r h2rr,
-specialize h2rr h4 h5, exact h2rr}, 
-{intros h1 y h5 h4, apply h1, intros z h6, specialize h4 z, apply h4, 
-specialize h2 a, cases h2 with h2l h2r, cases h2r with h2r h2rr, 
+{intros h1, apply h1, exact (h2 a).left x}, 
+{intros h1 y h4 z h5, apply h1 z,
+cases h2 a with h2l h2r, cases h2r with h2r h2rr,
+exact h2rr h4 h5}, 
+{intros h1 y h5 h4, apply h1, intros z h6, apply h4 z, 
+cases h2 a with h2l h2r, cases h2r with h2r h2rr, 
 exact h2rr (h2r h5) h6},
-{specialize ih_hp h3 x, specialize ih_hpq h3 x ih_hp, 
-exact ih_hpq},
+{exact ih_hpq h3 x (ih_hp h3 x)},
 {intros y h1, exact ih h3 y},
 {split, repeat {intros h1 h4, apply h1 h4}}, 
 {split, repeat {intros h1 h4, apply h1 h4}}, 
 {split, intros h1 h4 h5, exact (h1 h4) (h5 h4),
 intros h1 h4 h5, apply h1 h4, intro h6, exact h5}, 
 {split, intro h1, split, intro h4,
-specialize h1 h4, exact h1.left,
-intro h4, specialize h1 h4, exact h1.right, 
+exact (h1 h4).left,
+intro h4, exact (h1 h4).right, 
 intros h1 h4, split, exact h1.left h4, exact h1.right h4}, 
 {split, intros h1 h4 h5,
-specialize h4 h5, specialize h1 h5, apply h1, exact h4,
-intros h1 h4 h5, rw forcesPA at h1, rw forcesPA at h1,
-specialize h1 (λ h4, h5), rw forcesPA at h1, specialize h1 h4,
-exact h1},
+apply h1 h5, exact h4 h5,
+intros h1 h4 h5, exact h1 (λ h4, h5) h4},
 {split, rw forcesPA, rw public_announce_know, intro h1, exact h1,
 intro h1, rw public_announce_know, exact h1}, 
 {split, intro h1, rw compositionPA.public_announce_comp,
